<?xml version="1.0"?>
<rdf:RDF xmlns="http://purl.org/ai4st/ontology#"
     xml:base="http://purl.org/ai4st/ontology"
     xmlns:dc="http://purl.org/dc/elements/1.1/"
     xmlns:owl="http://www.w3.org/2002/07/owl#"
     xmlns:rdf="http://www.w3.org/1999/02/22-rdf-syntax-ns#"
     xmlns:xml="http://www.w3.org/XML/1998/namespace"
     xmlns:xsd="http://www.w3.org/2001/XMLSchema#"
     xmlns:rdfs="http://www.w3.org/2000/01/rdf-schema#"
     xmlns:skos="http://www.w3.org/2004/02/skos/core#"
     xmlns:vann="http://purl.org/vocab/vann/"
     xmlns:ai4st="http://purl.org/ai4st/ontology#"
     xmlns:papers="http://purl.org/ai4st/papers#"
     xmlns:dcterms="http://purl.org/dc/terms/"
     xmlns:ontology="http://purl.org/stc/ontology#"
     xmlns:new_terms="http://purl.org/ai4st/new_terms#">
    <owl:Ontology rdf:about="http://purl.org/ai4st/ontology#">
        <owl:versionIRI rdf:resource="http://purl.org/ai4st/ontology#/1.0.0"/>
        <owl:imports rdf:resource="http://purl.org/stc/ontology#/1.0.0"/>
        <dc:creator>Schieferdecker, Ina K.</dc:creator>
        <dc:title xml:lang="en">ai4st: The AI for ST taxonomy</dc:title>
        <dcterms:bibliographicCitation xml:lang="en">Schieferdecker, I.K.: &quot;ai4st: A taxonomy of research papers on the support of software testing (ST) through the use of artificial intelligence (AI) methods and techniques&quot;, 2025, http://purl.org/ai4st</dcterms:bibliographicCitation>
        <dcterms:license>http://creativecommons.org/licenses/by/4.0/legalcode.en</dcterms:license>
        <vann:preferredNamespacePrefix xml:lang="en">ai4st:</vann:preferredNamespacePrefix>
        <vann:preferredNamespaceUri>http://purl.org/ai4st/ontology</vann:preferredNamespaceUri>
        <rdfs:comment xml:lang="en">ai4st is a taxonomy for research papers on the use of artificial intelligence (AI) methods and techniques to support software testing (ST).  It relates papers to their topics and contributions. These contributions are categorised by the purpose of the solution aimed for, the ST activity or process targeted, the type of AI used and the level of automation supported.</rdfs:comment>
        <owl:versionInfo rdf:datatype="http://www.w3.org/2001/XMLSchema#integer">1</owl:versionInfo>
    </owl:Ontology>
    


    <!-- 
    ///////////////////////////////////////////////////////////////////////////////////////
    //
    // Annotation properties
    //
    ///////////////////////////////////////////////////////////////////////////////////////
     -->

    


    <!-- http://purl.org/dc/elements/1.1/creator -->

    <owl:AnnotationProperty rdf:about="http://purl.org/dc/elements/1.1/creator"/>
    


    <!-- http://purl.org/dc/elements/1.1/title -->

    <owl:AnnotationProperty rdf:about="http://purl.org/dc/elements/1.1/title"/>
    


    <!-- http://purl.org/dc/terms/bibliographicCitation -->

    <owl:AnnotationProperty rdf:about="http://purl.org/dc/terms/bibliographicCitation"/>
    


    <!-- http://purl.org/dc/terms/license -->

    <owl:AnnotationProperty rdf:about="http://purl.org/dc/terms/license"/>
    


    <!-- http://purl.org/vocab/vann/preferredNamespacePrefix -->

    <owl:AnnotationProperty rdf:about="http://purl.org/vocab/vann/preferredNamespacePrefix"/>
    


    <!-- http://purl.org/vocab/vann/preferredNamespaceUri -->

    <owl:AnnotationProperty rdf:about="http://purl.org/vocab/vann/preferredNamespaceUri"/>
    


    <!-- 
    ///////////////////////////////////////////////////////////////////////////////////////
    //
    // Object Properties
    //
    ///////////////////////////////////////////////////////////////////////////////////////
     -->

    


    <!-- http://purl.org/ai4st/ontology#belongsTo -->

    <owl:ObjectProperty rdf:about="http://purl.org/ai4st/ontology#belongsTo">
        <rdf:type rdf:resource="http://www.w3.org/2002/07/owl#AsymmetricProperty"/>
        <rdf:type rdf:resource="http://www.w3.org/2002/07/owl#TransitiveProperty"/>
        <rdf:type rdf:resource="http://www.w3.org/2002/07/owl#IrreflexiveProperty"/>
        <rdfs:domain rdf:resource="http://purl.org/nemo/gufo#AbstractIndividualType"/>
        <rdfs:range rdf:resource="http://purl.org/nemo/gufo#AbstractIndividualType"/>
    </owl:ObjectProperty>
    


    <!-- http://purl.org/ai4st/ontology#belongsToAIType -->

    <owl:ObjectProperty rdf:about="http://purl.org/ai4st/ontology#belongsToAIType">
        <rdfs:subPropertyOf rdf:resource="http://purl.org/ai4st/ontology#belongsTo"/>
        <rdf:type rdf:resource="http://www.w3.org/2002/07/owl#TransitiveProperty"/>
        <rdfs:domain rdf:resource="http://purl.org/ai4st/ontology#AIType"/>
        <rdfs:range rdf:resource="http://purl.org/ai4st/ontology#AIType"/>
    </owl:ObjectProperty>
    


    <!-- http://purl.org/ai4st/ontology#hasLevel -->

    <owl:ObjectProperty rdf:about="http://purl.org/ai4st/ontology#hasLevel">
        <rdfs:subPropertyOf rdf:resource="http://purl.org/nemo/gufo#hasAssociatedQualityValueType"/>
        <owl:inverseOf rdf:resource="http://purl.org/ai4st/ontology#levelEnabledBy"/>
        <rdfs:domain rdf:resource="http://purl.org/ai4st/ontology#ResearchPaper"/>
        <rdfs:range rdf:resource="http://purl.org/ai4st/ontology#AutomationLevel"/>
    </owl:ObjectProperty>
    


    <!-- http://purl.org/ai4st/ontology#hasParent -->

    <owl:ObjectProperty rdf:about="http://purl.org/ai4st/ontology#hasParent"/>
    


    <!-- http://purl.org/ai4st/ontology#hasPurpose -->

    <owl:ObjectProperty rdf:about="http://purl.org/ai4st/ontology#hasPurpose">
        <rdfs:subPropertyOf rdf:resource="http://purl.org/nemo/gufo#hasAssociatedQualityValueType"/>
        <owl:inverseOf rdf:resource="http://purl.org/ai4st/ontology#purposeAdressedBy"/>
        <rdfs:domain rdf:resource="http://purl.org/ai4st/ontology#ResearchPaper"/>
        <rdfs:range rdf:resource="http://purl.org/ai4st/ontology#SolutionPurpose"/>
    </owl:ObjectProperty>
    


    <!-- http://purl.org/ai4st/ontology#hasTarget -->

    <owl:ObjectProperty rdf:about="http://purl.org/ai4st/ontology#hasTarget">
        <rdfs:subPropertyOf rdf:resource="http://purl.org/nemo/gufo#hasAssociatedQualityValueType"/>
        <owl:inverseOf rdf:resource="http://purl.org/ai4st/ontology#targetFocussedBy"/>
        <rdfs:domain rdf:resource="http://purl.org/ai4st/ontology#ResearchPaper"/>
        <rdfs:range rdf:resource="http://purl.org/ai4st/ontology#Target"/>
    </owl:ObjectProperty>
    


    <!-- http://purl.org/ai4st/ontology#hasType -->

    <owl:ObjectProperty rdf:about="http://purl.org/ai4st/ontology#hasType">
        <rdfs:subPropertyOf rdf:resource="http://purl.org/nemo/gufo#hasAssociatedQualityValueType"/>
        <owl:inverseOf rdf:resource="http://purl.org/ai4st/ontology#typeUsedBy"/>
        <rdfs:domain rdf:resource="http://purl.org/ai4st/ontology#ResearchPaper"/>
        <rdfs:range rdf:resource="http://purl.org/ai4st/ontology#AIType"/>
    </owl:ObjectProperty>
    


    <!-- http://purl.org/ai4st/ontology#implementedIn -->

    <owl:ObjectProperty rdf:about="http://purl.org/ai4st/ontology#implementedIn">
        <rdfs:domain rdf:resource="http://purl.org/nemo/gufo#AbstractIndividualType"/>
        <rdfs:range rdf:resource="http://purl.org/nemo/gufo#EndurantType"/>
    </owl:ObjectProperty>
    


    <!-- http://purl.org/ai4st/ontology#isAboutResearchTopic -->

    <owl:ObjectProperty rdf:about="http://purl.org/ai4st/ontology#isAboutResearchTopic">
        <rdfs:subPropertyOf rdf:resource="http://purl.org/nemo/gufo#hasAssociatedQualityValueType"/>
        <owl:inverseOf rdf:resource="http://purl.org/ai4st/ontology#topicAddressedBy"/>
        <rdfs:domain rdf:resource="http://purl.org/ai4st/ontology#ResearchPaper"/>
        <rdfs:comment xml:lang="en">Represents the research topics that a research paper contributes to.</rdfs:comment>
        <rdfs:label>isAboutResearchTopic</rdfs:label>
    </owl:ObjectProperty>
    


    <!-- http://purl.org/ai4st/ontology#levelEnabledBy -->

    <owl:ObjectProperty rdf:about="http://purl.org/ai4st/ontology#levelEnabledBy">
        <rdfs:subPropertyOf rdf:resource="http://purl.org/ai4st/ontology#implementedIn"/>
        <rdfs:domain rdf:resource="http://purl.org/ai4st/ontology#AutomationLevel"/>
        <rdfs:range rdf:resource="http://purl.org/ai4st/ontology#ResearchPaper"/>
    </owl:ObjectProperty>
    


    <!-- http://purl.org/ai4st/ontology#purposeAdressedBy -->

    <owl:ObjectProperty rdf:about="http://purl.org/ai4st/ontology#purposeAdressedBy">
        <rdfs:subPropertyOf rdf:resource="http://purl.org/ai4st/ontology#implementedIn"/>
        <rdfs:domain rdf:resource="http://purl.org/ai4st/ontology#SolutionPurpose"/>
        <rdfs:range rdf:resource="http://purl.org/ai4st/ontology#ResearchPaper"/>
    </owl:ObjectProperty>
    


    <!-- http://purl.org/ai4st/ontology#targetFocussedBy -->

    <owl:ObjectProperty rdf:about="http://purl.org/ai4st/ontology#targetFocussedBy">
        <rdfs:subPropertyOf rdf:resource="http://purl.org/ai4st/ontology#implementedIn"/>
        <rdfs:domain rdf:resource="http://purl.org/ai4st/ontology#Target"/>
        <rdfs:range rdf:resource="http://purl.org/ai4st/ontology#ResearchPaper"/>
    </owl:ObjectProperty>
    


    <!-- http://purl.org/ai4st/ontology#topicAddressedBy -->

    <owl:ObjectProperty rdf:about="http://purl.org/ai4st/ontology#topicAddressedBy">
        <rdfs:subPropertyOf rdf:resource="http://purl.org/ai4st/ontology#implementedIn"/>
        <rdfs:range rdf:resource="http://purl.org/ai4st/ontology#ResearchPaper"/>
    </owl:ObjectProperty>
    


    <!-- http://purl.org/ai4st/ontology#typeUsedBy -->

    <owl:ObjectProperty rdf:about="http://purl.org/ai4st/ontology#typeUsedBy">
        <rdfs:subPropertyOf rdf:resource="http://purl.org/ai4st/ontology#implementedIn"/>
        <rdfs:domain rdf:resource="http://purl.org/ai4st/ontology#AIType"/>
        <rdfs:range rdf:resource="http://purl.org/ai4st/ontology#ResearchPaper"/>
    </owl:ObjectProperty>
    


    <!-- http://purl.org/nemo/gufo#hasAssociatedQualityValueType -->

    <owl:ObjectProperty rdf:about="http://purl.org/nemo/gufo#hasAssociatedQualityValueType"/>
    


    <!-- http://purl.org/nemo/gufo#isEventProperPartOf -->

    <owl:ObjectProperty rdf:about="http://purl.org/nemo/gufo#isEventProperPartOf"/>
    


    <!-- http://purl.org/nemo/gufo#mediates -->

    <owl:ObjectProperty rdf:about="http://purl.org/nemo/gufo#mediates"/>
    


    <!-- 
    ///////////////////////////////////////////////////////////////////////////////////////
    //
    // Classes
    //
    ///////////////////////////////////////////////////////////////////////////////////////
     -->

    


    <!-- http://purl.org/ai4st/ontology#AIType -->

    <owl:Class rdf:about="http://purl.org/ai4st/ontology#AIType">
        <rdfs:subClassOf rdf:resource="http://purl.org/nemo/gufo#AbstractIndividualType"/>
        <rdfs:comment xml:lang="en">Represents the type of the artificial intelligence (AI) system being used.

According to ISO/IEC 22989:2022 Information technology - Artificial intelligence - Artificial intelligence concepts and terminology, artificial intelligence (AI) is

- &lt;discipline&gt; research and development of mechanisms and applications of AI systems.

and

artificial intelligence system (AI system) is

- engineered system that generates outputs such as content, forecasts, recommendations or decisions for a given set of human-defined objectives.</rdfs:comment>
        <rdfs:label>Type of AI system</rdfs:label>
    </owl:Class>
    


    <!-- http://purl.org/ai4st/ontology#AutomationLevel -->

    <owl:Class rdf:about="http://purl.org/ai4st/ontology#AutomationLevel">
        <rdfs:subClassOf rdf:resource="http://purl.org/nemo/gufo#AbstractIndividualType"/>
        <rdfs:label>Level of AI automation</rdfs:label>
        <rdfs:label xml:lang="en">Represents the level of automation provided / enabled by the AI system being used.

According to ISO/IEC 22989:2022 Information technology - Artificial intelligence - Artificial intelligence concepts and terminology, artificial intelligence (AI) is

- &lt;discipline&gt; research and development of mechanisms and applications of AI systems.

and

artificial intelligence system (AI system) is

- engineered system that generates outputs such as content, forecasts, recommendations or decisions for a given set of human-defined objectives.</rdfs:label>
    </owl:Class>
    


    <!-- http://purl.org/ai4st/ontology#Model -->

    <owl:Class rdf:about="http://purl.org/ai4st/ontology#Model">
        <rdfs:subClassOf rdf:resource="http://purl.org/nemo/gufo#Mixin"/>
        <rdfs:comment xml:lang="en">Represents artifacts defining (semi-)formally (1) properties of one or more artefacts used by software engineering activities or processes or (2) properties of software engineering activities or processes.

According to ISO/IEC 22989:2022 Information technology - Artificial intelligence - Artificial intelligence concepts and terminology, model is

- physical, mathematical or otherwise logical representation of a system, entity, phenomenon, process or data.

Note: For the ai4st ontology, only mathematical or logical representations are relevant.</rdfs:comment>
        <rdfs:label>Model</rdfs:label>
    </owl:Class>
    


    <!-- http://purl.org/ai4st/ontology#ResearchPaper -->

    <owl:Class rdf:about="http://purl.org/ai4st/ontology#ResearchPaper">
        <rdfs:subClassOf rdf:resource="http://purl.org/nemo/gufo#Mixin"/>
        <rdfs:comment xml:lang="en">Represents an artifact documenting research findings like new insights, methods, techniques, etc.</rdfs:comment>
        <rdfs:label>ResearchPaper</rdfs:label>
    </owl:Class>
    


    <!-- http://purl.org/ai4st/ontology#SolutionPurpose -->

    <owl:Class rdf:about="http://purl.org/ai4st/ontology#SolutionPurpose">
        <rdfs:subClassOf rdf:resource="http://purl.org/nemo/gufo#AbstractIndividualType"/>
        <rdfs:comment xml:lang="en">Represents the purpose of using the AI system in a software development / operation processes or activities.</rdfs:comment>
        <rdfs:label>Solution purpose</rdfs:label>
    </owl:Class>
    


    <!-- http://purl.org/ai4st/ontology#Target -->

    <owl:Class rdf:about="http://purl.org/ai4st/ontology#Target">
        <rdfs:subClassOf rdf:resource="http://purl.org/nemo/gufo#AbstractIndividualType"/>
        <rdfs:comment xml:lang="en">Represents the primary concept, issue, component, software, or process in a software engineering process or activitiy being addressed.</rdfs:comment>
        <rdfs:label>Solution target</rdfs:label>
    </owl:Class>
    


    <!-- http://purl.org/nemo/gufo#AbstractIndividualType -->

    <owl:Class rdf:about="http://purl.org/nemo/gufo#AbstractIndividualType"/>
    


    <!-- http://purl.org/nemo/gufo#EndurantType -->

    <owl:Class rdf:about="http://purl.org/nemo/gufo#EndurantType"/>
    


    <!-- http://purl.org/nemo/gufo#Mixin -->

    <owl:Class rdf:about="http://purl.org/nemo/gufo#Mixin"/>
    


    <!-- https://purl.org/ai4st/ontology#Target -->

    <owl:Class rdf:about="https://purl.org/ai4st/ontology#Target"/>
    


    <!-- 
    ///////////////////////////////////////////////////////////////////////////////////////
    //
    // Individuals
    //
    ///////////////////////////////////////////////////////////////////////////////////////
     -->

    


    <!-- http://purl.org/ai4st/new_terms#visual_testing -->

    <owl:NamedIndividual rdf:about="http://purl.org/ai4st/new_terms#visual_testing">
        <rdf:type rdf:resource="https://purl.org/ai4st/ontology#Target"/>
        <hasParent rdf:resource="http://purl.org/stc/terms#interface_testing"/>
    </owl:NamedIndividual>
    


    <!-- http://purl.org/ai4st/ontology#AI-assisted_options -->

    <owl:NamedIndividual rdf:about="http://purl.org/ai4st/ontology#AI-assisted_options">
        <rdf:type rdf:resource="http://purl.org/ai4st/ontology#AutomationLevel"/>
        <rdfs:comment xml:lang="en">Represents the case in which choices, recommendations, or decision-support outputs for the target SE processes or activities are generated or enhanced by an AI system, while retaining human control over the final choice, recommendation or decision, which may differ from the AI outputs.</rdfs:comment>
        <rdfs:label>AI-assisted options</rdfs:label>
    </owl:NamedIndividual>
    


    <!-- http://purl.org/ai4st/ontology#AI-assisted_selection -->

    <owl:NamedIndividual rdf:about="http://purl.org/ai4st/ontology#AI-assisted_selection">
        <rdf:type rdf:resource="http://purl.org/ai4st/ontology#AutomationLevel"/>
        <rdfs:comment xml:lang="en">Represents the case in which choices, recommendations, or decision-support outputs for the target SE processes or activities are generated or enhanced by an AI system, where the final choices, recommendations or decisions require human confirmation and do not differ from the AI outputs.</rdfs:comment>
        <rdfs:label>AI-assisted selection</rdfs:label>
    </owl:NamedIndividual>
    


    <!-- http://purl.org/ai4st/ontology#AI-driven_full_automation -->

    <owl:NamedIndividual rdf:about="http://purl.org/ai4st/ontology#AI-driven_full_automation">
        <rdf:type rdf:resource="http://purl.org/ai4st/ontology#AutomationLevel"/>
        <rdfs:comment xml:lang="en">Represents the case in which AI is used to automate all tasks or decision-making components within the target SE processes or activities, without requiring human intervention.</rdfs:comment>
        <rdfs:label>AI-driven full automation</rdfs:label>
    </owl:NamedIndividual>
    


    <!-- http://purl.org/ai4st/ontology#AI-driven_partial_automation -->

    <owl:NamedIndividual rdf:about="http://purl.org/ai4st/ontology#AI-driven_partial_automation">
        <rdf:type rdf:resource="http://purl.org/ai4st/ontology#AutomationLevel"/>
        <rdfs:comment xml:lang="en">Represents the case in which AI is used to automate specific tasks or decision-making components within the target SE processes or activities, while other parts of the process remain under human control or require human intervention.</rdfs:comment>
        <rdfs:label>AI-driven partial automation</rdfs:label>
    </owl:NamedIndividual>
    


    <!-- http://purl.org/ai4st/ontology#Agentic_AI -->

    <owl:NamedIndividual rdf:about="http://purl.org/ai4st/ontology#Agentic_AI">
        <rdf:type rdf:resource="http://purl.org/ai4st/ontology#AIType"/>
        <rdfs:comment xml:lang="en">Represents AI systems that rely on autonomous agents using AI techniques to plan, adapt, and execute multi-step objectives with minimal human control.</rdfs:comment>
        <rdfs:label>Agentic AI</rdfs:label>
    </owl:NamedIndividual>
    


    <!-- http://purl.org/ai4st/ontology#Classical_machine_learning -->

    <owl:NamedIndividual rdf:about="http://purl.org/ai4st/ontology#Classical_machine_learning">
        <rdf:type rdf:resource="http://purl.org/ai4st/ontology#AIType"/>
        <belongsToAIType rdf:resource="http://purl.org/ai4st/ontology#Subsymbolic"/>
        <rdfs:comment xml:lang="en">Represents subsymbolic AI systems that rely on statistical and algorithmic learning techniques - such as decision trees, support vector machines, linear regression, and clustering - to learn patterns from structured data and make predictions or classifications. These models typically operate on explicitly defined features and do not involve deep neural networks.

This class of AI is used in contrast to deep learning AI.</rdfs:comment>
        <rdfs:label>Classical machine learning</rdfs:label>
    </owl:NamedIndividual>
    


    <!-- http://purl.org/ai4st/ontology#Deep_learning -->

    <owl:NamedIndividual rdf:about="http://purl.org/ai4st/ontology#Deep_learning">
        <rdf:type rdf:resource="http://purl.org/ai4st/ontology#AIType"/>
        <belongsToAIType rdf:resource="http://purl.org/ai4st/ontology#Subsymbolic"/>
        <rdfs:comment xml:lang="en">Represents subsymbolic AI systems that rely on deep artificial neural networks to automatically learn features and perform tasks such as classification or prediction, especially from large and complex datasets. 

According to ISO/IEC 22989:2022 Information technology - Artificial intelligence - Artificial intelligence concepts and terminology, deep learning (deep neural network learning) is

- AI approach to creating rich hierarchical representations through the training of neural networks with many hidden layers.</rdfs:comment>
        <rdfs:label>Deep learning AI</rdfs:label>
    </owl:NamedIndividual>
    


    <!-- http://purl.org/ai4st/ontology#ERP_system -->

    <owl:NamedIndividual rdf:about="http://purl.org/ai4st/ontology#ERP_system">
        <rdf:type rdf:resource="https://purl.org/ai4st/ontology#Target"/>
        <hasParent rdf:resource="http://purl.org/stc/terms#test_object"/>
    </owl:NamedIndividual>
    


    <!-- http://purl.org/ai4st/ontology#Evolutionary_algorithms -->

    <owl:NamedIndividual rdf:about="http://purl.org/ai4st/ontology#Evolutionary_algorithms">
        <rdf:type rdf:resource="http://purl.org/ai4st/ontology#AIType"/>
        <belongsToAIType rdf:resource="http://purl.org/ai4st/ontology#Subsymbolic"/>
    </owl:NamedIndividual>
    


    <!-- http://purl.org/ai4st/ontology#General_AI -->

    <owl:NamedIndividual rdf:about="http://purl.org/ai4st/ontology#General_AI">
        <rdf:type rdf:resource="http://purl.org/ai4st/ontology#AIType"/>
        <rdfs:comment xml:lang="en">Represents AI systems capable of performing a broad set of distinct tasks with satisfactory performance.

According to ISO/IEC 22989:2022 Information technology - Artificial intelligence - Artificial intelligence concepts and terminology, general AI (AGI, artificial general intelligence)

- type of AI system that addresses a broad range of tasks with a satisfactory level of performance 

Note 1: Compared to narrow AI.
Note 2: AGI is often used in a stronger sense, meaning systems that not only can perform a wide variety of tasks, but all tasks that a human can perform.</rdfs:comment>
        <rdfs:label>General AI</rdfs:label>
    </owl:NamedIndividual>
    


    <!-- http://purl.org/ai4st/ontology#Generate -->

    <owl:NamedIndividual rdf:about="http://purl.org/ai4st/ontology#Generate">
        <rdf:type rdf:resource="http://purl.org/ai4st/ontology#SolutionPurpose"/>
    </owl:NamedIndividual>
    


    <!-- http://purl.org/ai4st/ontology#Generative_AI -->

    <owl:NamedIndividual rdf:about="http://purl.org/ai4st/ontology#Generative_AI">
        <rdf:type rdf:resource="http://purl.org/ai4st/ontology#AIType"/>
        <rdfs:comment xml:lang="en">Represents AI systems that use learned or derived knowledge to produce original outputs, such as synthetic text, media, or other content types. It often uses subsymbolic AI like Convolutional Neural Networks (CNNs), Recurrent Neural Networks (RNNs), or Transformer-based models, but also symbolic AI.</rdfs:comment>
        <rdfs:label>Generative AI</rdfs:label>
    </owl:NamedIndividual>
    


    <!-- http://purl.org/ai4st/ontology#Improve -->

    <owl:NamedIndividual rdf:about="http://purl.org/ai4st/ontology#Improve">
        <rdf:type rdf:resource="http://purl.org/ai4st/ontology#SolutionPurpose"/>
        <rdfs:comment xml:lang="en">The purpose of using AI is to improve (parts of) artefacts used in software engineering.</rdfs:comment>
        <rdfs:label>Improve</rdfs:label>
    </owl:NamedIndividual>
    


    <!-- http://purl.org/ai4st/ontology#No_AI_automation -->

    <owl:NamedIndividual rdf:about="http://purl.org/ai4st/ontology#No_AI_automation">
        <rdf:type rdf:resource="http://purl.org/ai4st/ontology#AutomationLevel"/>
        <rdfs:comment xml:lang="en">Represents the case in which the target SE processes or activities are performed without the assistance of AI.</rdfs:comment>
        <rdfs:label>No AI-supported automation</rdfs:label>
    </owl:NamedIndividual>
    


    <!-- http://purl.org/ai4st/ontology#Statistical -->

    <owl:NamedIndividual rdf:about="http://purl.org/ai4st/ontology#Statistical">
        <rdf:type rdf:resource="http://purl.org/ai4st/ontology#AIType"/>
        <belongsToAIType rdf:resource="http://purl.org/ai4st/ontology#Subsymbolic"/>
        <rdfs:comment xml:lang="en">Represents subsymbolic AI systems that rely on data and statistical inference to identify patterns and make predictions.</rdfs:comment>
        <rdfs:label>Statistical AI</rdfs:label>
    </owl:NamedIndividual>
    


    <!-- http://purl.org/ai4st/ontology#Subsymbolic -->

    <owl:NamedIndividual rdf:about="http://purl.org/ai4st/ontology#Subsymbolic">
        <rdf:type rdf:resource="http://purl.org/ai4st/ontology#AIType"/>
        <rdfs:comment xml:lang="en">Represents AI systems that use numerical models to represent knowledge and computations, such as numerical optimisation and statistical learning, in order to model and solve problems.

According to ISO/IEC 22989:2022 Information technology - Artificial intelligence - Artificial intelligence concepts and terminology, subsymbolic AI is

- AI based on techniques and models that use an implicit encoding of information, that can be derived from experience or raw data.</rdfs:comment>
        <rdfs:label>Subsymbolic AI</rdfs:label>
    </owl:NamedIndividual>
    


    <!-- http://purl.org/ai4st/ontology#Swarm_intelligence -->

    <owl:NamedIndividual rdf:about="http://purl.org/ai4st/ontology#Swarm_intelligence">
        <rdf:type rdf:resource="http://purl.org/ai4st/ontology#AIType"/>
        <belongsToAIType rdf:resource="http://purl.org/ai4st/ontology#Subsymbolic"/>
    </owl:NamedIndividual>
    


    <!-- http://purl.org/ai4st/ontology#Symbolic -->

    <owl:NamedIndividual rdf:about="http://purl.org/ai4st/ontology#Symbolic">
        <rdf:type rdf:resource="http://purl.org/ai4st/ontology#AIType"/>
        <rdfs:comment xml:lang="en">Represents AI systems that use approaches relying on the explicit definition of symbols and rules representing knowledge and performing logical reasoning.

According to ISO/IEC 22989:2022 Information technology - Artificial intelligence - Artificial intelligence concepts and terminology, symbolic AI is

- AI based on techniques and models that manipulate symbols and structures according to explicitly defined rules to obtain inferences.</rdfs:comment>
        <rdfs:label>Symbolic AI</rdfs:label>
    </owl:NamedIndividual>
    


    <!-- http://purl.org/ai4st/ontology#Understand -->

    <owl:NamedIndividual rdf:about="http://purl.org/ai4st/ontology#Understand">
        <rdf:type rdf:resource="http://purl.org/ai4st/ontology#SolutionPurpose"/>
        <rdfs:comment xml:lang="en">The purpose of using AI is to gain insight.</rdfs:comment>
        <rdfs:label>Understand</rdfs:label>
    </owl:NamedIndividual>
    


    <!-- http://purl.org/ai4st/ontology#Web_application -->

    <owl:NamedIndividual rdf:about="http://purl.org/ai4st/ontology#Web_application">
        <rdf:type rdf:resource="https://purl.org/ai4st/ontology#Target"/>
        <hasParent rdf:resource="http://purl.org/stc/terms#test_object"/>
    </owl:NamedIndividual>
    


    <!-- http://purl.org/ai4st/ontology#assertion -->

    <owl:NamedIndividual rdf:about="http://purl.org/ai4st/ontology#assertion">
        <rdf:type rdf:resource="https://purl.org/ai4st/ontology#Target"/>
        <hasParent rdf:resource="http://purl.org/stc/terms#Testware"/>
    </owl:NamedIndividual>
    


    <!-- http://purl.org/ai4st/ontology#computer_game -->

    <owl:NamedIndividual rdf:about="http://purl.org/ai4st/ontology#computer_game">
        <rdf:type rdf:resource="https://purl.org/ai4st/ontology#Target"/>
        <hasParent rdf:resource="http://purl.org/stc/terms#test_object"/>
    </owl:NamedIndividual>
    


    <!-- http://purl.org/ai4st/ontology#concolic_testing -->

    <owl:NamedIndividual rdf:about="http://purl.org/ai4st/ontology#concolic_testing">
        <rdf:type rdf:resource="https://purl.org/ai4st/ontology#Target"/>
        <hasParent rdf:resource="http://purl.org/stc/terms#white_box_test_technique"/>
    </owl:NamedIndividual>
    


    <!-- http://purl.org/ai4st/ontology#ethics -->

    <owl:NamedIndividual rdf:about="http://purl.org/ai4st/ontology#ethics">
        <rdf:type rdf:resource="https://purl.org/ai4st/ontology#Target"/>
        <hasParent rdf:resource="http://purl.org/stc/terms#basic_concepts"/>
    </owl:NamedIndividual>
    


    <!-- http://purl.org/ai4st/ontology#mutation_testing -->

    <owl:NamedIndividual rdf:about="http://purl.org/ai4st/ontology#mutation_testing">
        <rdf:type rdf:resource="https://purl.org/ai4st/ontology#Target"/>
        <hasParent rdf:resource="http://purl.org/stc/terms#white_box_test_technique"/>
    </owl:NamedIndividual>
    


    <!-- http://purl.org/ai4st/ontology#null -->

    <owl:Thing rdf:about="http://purl.org/ai4st/ontology#null">
        <rdf:type rdf:resource="http://www.w3.org/2002/07/owl#NamedIndividual"/>
    </owl:Thing>
    


    <!-- http://purl.org/ai4st/ontology#penetration_testing -->

    <owl:NamedIndividual rdf:about="http://purl.org/ai4st/ontology#penetration_testing">
        <rdf:type rdf:resource="https://purl.org/ai4st/ontology#Target"/>
        <hasParent rdf:resource="http://purl.org/stc/terms#security_testing"/>
    </owl:NamedIndividual>
    


    <!-- http://purl.org/ai4st/ontology#test_documentation -->

    <owl:NamedIndividual rdf:about="http://purl.org/ai4st/ontology#test_documentation">
        <rdf:type rdf:resource="https://purl.org/ai4st/ontology#Target"/>
        <hasParent rdf:resource="http://purl.org/stc/terms#test_activity"/>
    </owl:NamedIndividual>
    


    <!-- http://purl.org/ai4st/ontology#test_generation -->

    <owl:NamedIndividual rdf:about="http://purl.org/ai4st/ontology#test_generation">
        <rdf:type rdf:resource="https://purl.org/ai4st/ontology#Target"/>
        <hasParent rdf:resource="http://purl.org/stc/terms#test_activity"/>
    </owl:NamedIndividual>
    


    <!-- http://purl.org/ai4st/ontology#test_prioritization -->

    <owl:NamedIndividual rdf:about="http://purl.org/ai4st/ontology#test_prioritization">
        <rdf:type rdf:resource="https://purl.org/ai4st/ontology#Target"/>
        <hasParent rdf:resource="http://purl.org/stc/terms#test_activity"/>
    </owl:NamedIndividual>
    


    <!-- http://purl.org/ai4st/ontology#test_selection -->

    <owl:NamedIndividual rdf:about="http://purl.org/ai4st/ontology#test_selection">
        <rdf:type rdf:resource="https://purl.org/ai4st/ontology#Target"/>
        <hasParent rdf:resource="http://purl.org/stc/terms#test_execution"/>
    </owl:NamedIndividual>
    


    <!-- http://purl.org/ai4st/ontology#test_verification -->

    <owl:NamedIndividual rdf:about="http://purl.org/ai4st/ontology#test_verification">
        <rdf:type rdf:resource="https://purl.org/ai4st/ontology#Target"/>
        <hasParent rdf:resource="http://purl.org/stc/terms#test_activity"/>
    </owl:NamedIndividual>
    


    <!-- http://purl.org/ai4st/ontology#CSO:Testing_and_Debugging -->

    <owl:NamedIndividual rdf:about="http://purl.org/ai4st/ontology#CSO:Testing_and_Debugging"/>
    


    <!-- http://purl.org/ai4st/papers#abdelkarim_tcp-net_2023 -->

    <owl:NamedIndividual rdf:about="http://purl.org/ai4st/papers#abdelkarim_tcp-net_2023">
        <rdf:type rdf:resource="http://purl.org/ai4st/ontology#ResearchPaper"/>
        <hasLevel rdf:resource="http://purl.org/ai4st/ontology#AI-assisted_options"/>
        <hasPurpose rdf:resource="http://purl.org/ai4st/ontology#Generate"/>
        <hasTarget rdf:resource="http://purl.org/ai4st/ontology#test_prioritization"/>
        <hasType rdf:resource="http://purl.org/ai4st/ontology#Deep_learning"/>
        <isAboutResearchTopic rdf:resource="http://purl.org/ai4st/ontology#CSO:Testing_and_Debugging"/>
        <rdfs:comment>@inproceedings{abdelkarim_tcp-net_2023,
 address = {Athens, Greece},
 author = {Abdelkarim, Mohamed and ElAdawi, Reem},
 booktitle = {2023 {IEEE} {International} {Conference} {On} {Artificial} {Intelligence} {Testing} ({AITest})},
 copyright = {http://doi.org/10.15223/policy-029},
 doi = {10.1109/AITest58265.2023.00024},
 isbn = {979-8-3503-3629-0},
 month = {July},
 pages = {99--106},
 publisher = {IEEE},
 shorttitle = {{TCP}-{Net}++},
 title = {{TCP}-{Net}++: {Test} {Case} {Prioritization} {Using} {End}-to-{End} {Deep} {Neural} {Networks} - {Deployment} {Analysis} and {Enhancements}},
 url = {http://ieeexplore.ieee.org/document/10229439/},
 urldate = {2025-06-12},
 year = {2023}
}
</rdfs:comment>
        <rdfs:label>abdelkarim_tcp-net_2023</rdfs:label>
        <rdfs:seeAlso rdf:resource="http://ieeexplore.ieee.org/document/10229439/"/>
    </owl:NamedIndividual>
    


    <!-- http://purl.org/ai4st/papers#caglar_development_2023 -->

    <owl:NamedIndividual rdf:about="http://purl.org/ai4st/papers#caglar_development_2023">
        <rdf:type rdf:resource="http://purl.org/ai4st/ontology#ResearchPaper"/>
        <hasLevel rdf:resource="http://purl.org/ai4st/ontology#AI-driven_full_automation"/>
        <hasPurpose rdf:resource="http://purl.org/ai4st/ontology#Generate"/>
        <hasTarget rdf:resource="http://purl.org/ai4st/ontology#mutation_testing"/>
        <hasType rdf:resource="http://purl.org/ai4st/ontology#Deep_learning"/>
        <isAboutResearchTopic rdf:resource="http://purl.org/ai4st/ontology#CSO:Testing_and_Debugging"/>
        <rdfs:comment>@inproceedings{caglar_development_2023,
 address = {Sivas, Turkiye},
 author = {Caglar, Osman and Taskin, Furkan and Baglum, Cem and Asik, Sergen and Yayan, Ugur},
 booktitle = {2023 {Innovations} in {Intelligent} {Systems} and {Applications} {Conference} ({ASYU})},
 copyright = {http://doi.org/10.15223/policy-029},
 doi = {10.1109/ASYU58738.2023.10296551},
 isbn = {979-8-3503-0659-0},
 month = {October},
 pages = {1--6},
 publisher = {IEEE},
 title = {Development of {Cloud} and {Artificial} {Intelligence} based {Software} {Testing} {Platform} ({ChArIoT})},
 url = {http://ieeexplore.ieee.org/document/10296551/},
 urldate = {2025-06-12},
 year = {2023}
}
</rdfs:comment>
        <rdfs:label>caglar_development_2023</rdfs:label>
        <rdfs:seeAlso rdf:resource="http://ieeexplore.ieee.org/document/10296551/"/>
    </owl:NamedIndividual>
    


    <!-- http://purl.org/ai4st/papers#calvano_leveraging_2025 -->

    <owl:NamedIndividual rdf:about="http://purl.org/ai4st/papers#calvano_leveraging_2025">
        <rdf:type rdf:resource="http://purl.org/ai4st/ontology#ResearchPaper"/>
        <hasLevel rdf:resource="http://purl.org/ai4st/ontology#AI-assisted_options"/>
        <hasPurpose rdf:resource="http://purl.org/ai4st/ontology#Generate"/>
        <hasTarget rdf:resource="http://purl.org/stc/terms#usability_testing"/>
        <hasType rdf:resource="http://purl.org/ai4st/ontology#Generative_AI"/>
        <isAboutResearchTopic rdf:resource="http://purl.org/ai4st/ontology#CSO:Testing_and_Debugging"/>
        <rdfs:comment>@inproceedings{calvano_leveraging_2025,
 address = {Cagliari Italy},
 author = {Calvano, Miriana and Curci, Antonio and Lanzilotti, Rosa and Piccinno, Antonio and Ragone, Azzurra},
 booktitle = {Companion {Proceedings} of the 30th {International} {Conference} on {Intelligent} {User} {Interfaces}},
 doi = {10.1145/3708557.3716341},
 isbn = {979-8-4007-1409-2},
 language = {en},
 month = {March},
 pages = {78--81},
 publisher = {ACM},
 shorttitle = {Leveraging {Large} {Language} {Models} for {Usability} {Testing}},
 title = {Leveraging {Large} {Language} {Models} for {Usability} {Testing}: a {Preliminary} {Study}},
 url = {http://dl.acm.org/doi/10.1145/3708557.3716341},
 urldate = {2025-06-12},
 year = {2025}
}
</rdfs:comment>
        <rdfs:label>calvano_leveraging_2025</rdfs:label>
        <rdfs:seeAlso rdf:resource="http://dl.acm.org/doi/10.1145/3708557.3716341"/>
    </owl:NamedIndividual>
    


    <!-- http://purl.org/ai4st/papers#confido_reinforcing_2022 -->

    <owl:NamedIndividual rdf:about="http://purl.org/ai4st/papers#confido_reinforcing_2022">
        <rdf:type rdf:resource="http://purl.org/ai4st/ontology#ResearchPaper"/>
        <hasLevel rdf:resource="http://purl.org/ai4st/ontology#AI-driven_full_automation"/>
        <hasPurpose rdf:resource="http://purl.org/ai4st/ontology#Improve"/>
        <hasTarget rdf:resource="http://purl.org/ai4st/ontology#penetration_testing"/>
        <hasType rdf:resource="http://purl.org/ai4st/ontology#Deep_learning"/>
        <isAboutResearchTopic rdf:resource="http://purl.org/ai4st/ontology#CSO:Testing_and_Debugging"/>
        <rdfs:comment>@inproceedings{confido_reinforcing_2022,
 address = {Big Sky, MT, USA},
 author = {Confido, Alessandro and Ntagiou, Evridiki V. and Wallum, Marcus},
 booktitle = {2022 {IEEE} {Aerospace} {Conference} ({AERO})},
 copyright = {http://doi.org/10.15223/policy-029},
 doi = {10.1109/AERO53065.2022.9843459},
 isbn = {978-1-6654-3760-8},
 month = {March},
 pages = {1--15},
 publisher = {IEEE},
 title = {Reinforcing {Penetration} {Testing} {Using} {AI}},
 url = {http://ieeexplore.ieee.org/document/9843459/},
 urldate = {2025-06-12},
 year = {2022}
}
</rdfs:comment>
        <rdfs:label>confido_reinforcing_2022</rdfs:label>
        <rdfs:seeAlso rdf:resource="http://ieeexplore.ieee.org/document/9843459/"/>
    </owl:NamedIndividual>
    


    <!-- http://purl.org/ai4st/papers#de_almeida_ai_2024 -->

    <owl:NamedIndividual rdf:about="http://purl.org/ai4st/papers#de_almeida_ai_2024">
        <rdf:type rdf:resource="http://purl.org/ai4st/ontology#ResearchPaper"/>
        <hasLevel rdf:resource="http://purl.org/ai4st/ontology#AI-assisted_options"/>
        <hasPurpose rdf:resource="http://purl.org/ai4st/ontology#Generate"/>
        <hasTarget rdf:resource="http://purl.org/stc/terms#exploratory_testing"/>
        <hasType rdf:resource="http://purl.org/ai4st/ontology#Generative_AI"/>
        <isAboutResearchTopic rdf:resource="http://purl.org/ai4st/ontology#CSO:Testing_and_Debugging"/>
        <rdfs:comment>@inproceedings{de_almeida_ai_2024,
 address = {Salvador Bahia Brazil},
 author = {De Almeida, Ágatha and Collins, Eliane and Oran, Ana Carolina},
 booktitle = {Proceedings of the {XXIII} {Brazilian} {Symposium} on {Software} {Quality}},
 doi = {10.1145/3701625.3701657},
 isbn = {979-8-4007-1777-2},
 language = {en},
 month = {November},
 pages = {179--188},
 publisher = {ACM},
 shorttitle = {{AI} in {Service} of {Software} {Quality}},
 title = {{AI} in {Service} of {Software} {Quality}: {How} {ChatGPT} and {Personas} {Are} {Transforming} {Exploratory} {Testing}},
 url = {http://dl.acm.org/doi/10.1145/3701625.3701657},
 urldate = {2025-06-12},
 year = {2024}
}
</rdfs:comment>
        <rdfs:label>de_almeida_ai_2024</rdfs:label>
        <rdfs:seeAlso rdf:resource="http://dl.acm.org/doi/10.1145/3701625.3701657"/>
    </owl:NamedIndividual>
    


    <!-- http://purl.org/ai4st/papers#de_santiago_junior_method_2022 -->

    <owl:NamedIndividual rdf:about="http://purl.org/ai4st/papers#de_santiago_junior_method_2022">
        <rdf:type rdf:resource="http://purl.org/ai4st/ontology#ResearchPaper"/>
        <hasLevel rdf:resource="http://purl.org/ai4st/ontology#AI-assisted_options"/>
        <hasPurpose rdf:resource="http://purl.org/ai4st/ontology#Generate"/>
        <hasTarget rdf:resource="http://purl.org/stc/terms#test_oracle"/>
        <hasType rdf:resource="http://purl.org/ai4st/ontology#Deep_learning"/>
        <isAboutResearchTopic rdf:resource="http://purl.org/ai4st/ontology#CSO:Testing_and_Debugging"/>
        <rdfs:comment>@inproceedings{de_santiago_junior_method_2022,
 address = {Pittsburgh Pennsylvania},
 author = {De Santiago Júnior, Valdivino Alexandre},
 booktitle = {Proceedings of the 3rd {ACM}/{IEEE} {International} {Conference} on {Automation} of {Software} {Test}},
 doi = {10.1145/3524481.3527232},
 isbn = {978-1-4503-9286-0},
 language = {en},
 month = {May},
 pages = {40--51},
 publisher = {ACM},
 title = {A method and experiment to evaluate deep neural networks as test oracles for scientific software},
 url = {http://dl.acm.org/doi/10.1145/3524481.3527232},
 urldate = {2025-06-12},
 year = {2022}
}
</rdfs:comment>
        <rdfs:label>de_santiago_junior_method_2022</rdfs:label>
        <rdfs:seeAlso rdf:resource="http://dl.acm.org/doi/10.1145/3524481.3527232"/>
    </owl:NamedIndividual>
    


    <!-- http://purl.org/ai4st/papers#djajadi_using_nodate -->

    <owl:NamedIndividual rdf:about="http://purl.org/ai4st/papers#djajadi_using_nodate">
        <rdf:type rdf:resource="http://purl.org/ai4st/ontology#ResearchPaper"/>
        <hasLevel rdf:resource="http://purl.org/ai4st/ontology#AI-assisted_options"/>
        <hasPurpose rdf:resource="http://purl.org/ai4st/ontology#Generate"/>
        <hasPurpose rdf:resource="http://purl.org/ai4st/ontology#Understand"/>
        <hasTarget rdf:resource="http://purl.org/ai4st/ontology#test_documentation"/>
        <hasType rdf:resource="http://purl.org/ai4st/ontology#Generative_AI"/>
        <isAboutResearchTopic rdf:resource="http://purl.org/ai4st/ontology#CSO:Testing_and_Debugging"/>
        <rdfs:comment>@inproceedings{djajadi_using_nodate,
 author = {Djajadi, Natanael and Deljouyi, Amirhossein and Zaidman, Andy},
 booktitle = {Early {Research} {Achievements} ({ERA})},
 doi = {10.1109/ICPC66645.2025.00040},
 title = {Using {Large} {Language} {Models} to {Generate} {Concise} and {Understandable} {Test} {Case} {Summaries}},
 url = {http://azaidman.github.io/publications/djajadiICPC2025.pdf},
 urldate = {2025-06-12}
}</rdfs:comment>
        <rdfs:label>djajadi_using_nodate</rdfs:label>
        <rdfs:seeAlso rdf:resource="http://azaidman.github.io/publications/djajadiICPC2025.pdf"/>
    </owl:NamedIndividual>
    


    <!-- http://purl.org/ai4st/papers#ferreira_acceptance_2025 -->

    <owl:NamedIndividual rdf:about="http://purl.org/ai4st/papers#ferreira_acceptance_2025">
        <rdf:type rdf:resource="http://purl.org/ai4st/ontology#ResearchPaper"/>
        <hasLevel rdf:resource="http://purl.org/ai4st/ontology#AI-assisted_selection"/>
        <hasPurpose rdf:resource="http://purl.org/ai4st/ontology#Generate"/>
        <hasTarget rdf:resource="http://purl.org/ai4st/ontology#Web_application"/>
        <hasTarget rdf:resource="http://purl.org/stc/terms#acceptance_testing"/>
        <hasTarget rdf:resource="http://purl.org/stc/terms#test_automation"/>
        <hasType rdf:resource="http://purl.org/ai4st/ontology#Generative_AI"/>
        <isAboutResearchTopic rdf:resource="http://purl.org/ai4st/ontology#CSO:Testing_and_Debugging"/>
        <rdfs:comment>@misc{ferreira_acceptance_2025,
 author = {Ferreira, Margarida and Viegas, Luis and Faria, Joao Pascoal and Lima, Bruno},
 doi = {10.48550/arXiv.2504.07244},
 keywords = {Computer Science - Software Engineering},
 month = {April},
 note = {arXiv:2504.07244 [cs]},
 publisher = {arXiv},
 shorttitle = {Acceptance {Test} {Generation} with {Large} {Language} {Models}},
 title = {Acceptance {Test} {Generation} with {Large} {Language} {Models}: {An} {Industrial} {Case} {Study}},
 url = {http://arxiv.org/abs/2504.07244},
 urldate = {2025-06-12},
 year = {2025}
}</rdfs:comment>
        <rdfs:label>ferreira_acceptance_2025</rdfs:label>
        <rdfs:seeAlso rdf:resource="http://arxiv.org/abs/2504.07244"/>
    </owl:NamedIndividual>
    


    <!-- http://purl.org/ai4st/papers#franzosi_llm-based_2025 -->

    <owl:NamedIndividual rdf:about="http://purl.org/ai4st/papers#franzosi_llm-based_2025">
        <rdf:type rdf:resource="http://purl.org/ai4st/ontology#ResearchPaper"/>
        <hasLevel rdf:resource="http://purl.org/ai4st/ontology#AI-driven_partial_automation"/>
        <hasPurpose rdf:resource="http://purl.org/ai4st/ontology#Generate"/>
        <hasTarget rdf:resource="http://purl.org/stc/terms#GUI_testing"/>
        <hasTarget rdf:resource="http://purl.org/stc/terms#test_report"/>
        <hasType rdf:resource="http://purl.org/ai4st/ontology#Generative_AI"/>
        <isAboutResearchTopic rdf:resource="http://purl.org/ai4st/ontology#CSO:Testing_and_Debugging"/>
        <rdfs:comment>@inproceedings{franzosi_llm-based_2025,
 address = {Napoli, Italy},
 author = {Franzosi, Diogo Buarque and Alégroth, Emil and Isaac, Maycel},
 booktitle = {2025 {IEEE} {Conference} on {Software} {Testing}, {Verification} and {Validation} ({ICST})},
 copyright = {http://doi.org/10.15223/policy-029},
 doi = {10.1109/ICST62969.2025.10988984},
 isbn = {979-8-3315-0814-2},
 month = {March},
 pages = {453--463},
 publisher = {IEEE},
 title = {{LLM}-{Based} {Labelling} of {Recorded} {Automated} {GUI}-{Based} {Test} {Cases}},
 url = {http://ieeexplore.ieee.org/document/10988984/},
 urldate = {2025-06-12},
 year = {2025}
}
</rdfs:comment>
        <rdfs:label>franzosi_llm-based_2025</rdfs:label>
        <rdfs:seeAlso rdf:resource="http://ieeexplore.ieee.org/document/10988984/"/>
    </owl:NamedIndividual>
    


    <!-- http://purl.org/ai4st/papers#gamal_owl_2023 -->

    <owl:NamedIndividual rdf:about="http://purl.org/ai4st/papers#gamal_owl_2023">
        <rdf:type rdf:resource="http://purl.org/ai4st/ontology#ResearchPaper"/>
        <hasLevel rdf:resource="http://purl.org/ai4st/ontology#AI-driven_full_automation"/>
        <hasPurpose rdf:resource="http://purl.org/ai4st/ontology#Generate"/>
        <hasTarget rdf:resource="http://purl.org/ai4st/new_terms#visual_testing"/>
        <hasTarget rdf:resource="http://purl.org/stc/terms#GUI_testing"/>
        <hasType rdf:resource="http://purl.org/ai4st/ontology#Deep_learning"/>
        <isAboutResearchTopic rdf:resource="http://purl.org/ai4st/ontology#CSO:Testing_and_Debugging"/>
        <rdfs:comment>@inproceedings{gamal_owl_2023,
 address = {Giza, Egypt},
 author = {Gamal, Ahmed and Emad, Reem and Mohamed, Taher and Mohamed, Omar and Hamdy, Ahmed and Ali, Sarah},
 booktitle = {2023 5th {Novel} {Intelligent} and {Leading} {Emerging} {Sciences} {Conference} ({NILES})},
 copyright = {http://doi.org/10.15223/policy-029},
 doi = {10.1109/NILES59815.2023.10296575},
 isbn = {979-8-3503-8103-0},
 month = {October},
 pages = {312--315},
 publisher = {IEEE},
 shorttitle = {Owl {Eye}},
 title = {Owl {Eye}: {An} {AI}-{Driven} {Visual} {Testing} {Tool}},
 url = {http://ieeexplore.ieee.org/document/10296575/},
 urldate = {2025-06-12},
 year = {2023}
}
</rdfs:comment>
        <rdfs:label>gamal_owl_2023</rdfs:label>
        <rdfs:seeAlso rdf:resource="http://ieeexplore.ieee.org/document/10296575/"/>
    </owl:NamedIndividual>
    


    <!-- http://purl.org/ai4st/papers#gao_approach_2022 -->

    <owl:NamedIndividual rdf:about="http://purl.org/ai4st/papers#gao_approach_2022">
        <rdf:type rdf:resource="http://purl.org/ai4st/ontology#ResearchPaper"/>
        <hasLevel rdf:resource="http://purl.org/ai4st/ontology#AI-assisted_selection"/>
        <hasPurpose rdf:resource="http://purl.org/ai4st/ontology#Generate"/>
        <hasTarget rdf:resource="http://purl.org/stc/terms#GUI_testing"/>
        <hasType rdf:resource="http://purl.org/ai4st/ontology#Deep_learning"/>
        <isAboutResearchTopic rdf:resource="http://purl.org/ai4st/ontology#CSO:Testing_and_Debugging"/>
        <rdfs:comment>@inproceedings{gao_approach_2022,
 address = {Newark, CA, USA},
 author = {Gao, Jerry and Li, ShiTing and Tao, Chuanqi and He, Yejun and Anumalasetty, Amrutha Pavani and Joseph, Erica Wilson and Sripathi, Akshata Hatwar Kumbashi and Nayani, Himabindu},
 booktitle = {2022 {IEEE} {International} {Conference} {On} {Artificial} {Intelligence} {Testing} ({AITest})},
 copyright = {http://doi.org/10.15223/policy-029},
 doi = {10.1109/AITest55621.2022.00020},
 isbn = {978-1-6654-8737-5},
 month = {August},
 pages = {79--86},
 publisher = {IEEE},
 title = {An {Approach} to {GUI} {Test} {Scenario} {Generation} {Using} {Machine} {Learning}},
 url = {http://ieeexplore.ieee.org/document/9898132/},
 urldate = {2025-06-12},
 year = {2022}
}
</rdfs:comment>
        <rdfs:label>gao_approach_2022</rdfs:label>
        <rdfs:seeAlso rdf:resource="http://ieeexplore.ieee.org/document/9898132/"/>
    </owl:NamedIndividual>
    


    <!-- http://purl.org/ai4st/papers#gao_clozemaster_2025 -->

    <owl:NamedIndividual rdf:about="http://purl.org/ai4st/papers#gao_clozemaster_2025">
        <rdf:type rdf:resource="http://purl.org/ai4st/ontology#ResearchPaper"/>
        <hasLevel rdf:resource="http://purl.org/ai4st/ontology#AI-driven_full_automation"/>
        <hasPurpose rdf:resource="http://purl.org/ai4st/ontology#Generate"/>
        <hasTarget rdf:resource="http://purl.org/ai4st/ontology#test_generation"/>
        <hasType rdf:resource="http://purl.org/ai4st/ontology#Generative_AI"/>
        <isAboutResearchTopic rdf:resource="http://purl.org/ai4st/ontology#CSO:Testing_and_Debugging"/>
        <rdfs:comment>@inproceedings{gao_clozemaster_2025,
 author = {Gao, Hongyan and Yang, Yibiao and Sun, Maolin and Wu, Jiangchang and Zhou, Yuming and Xu, Baowen},
 doi = {10.1109/ICSE55347.2025.00175},
 isbn = {979-8-3315-0569-1},
 language = {English},
 month = {March},
 note = {ISSN: 1558-1225},
 pages = {712--712},
 publisher = {IEEE Computer Society},
 shorttitle = {{ClozeMaster}},
 title = {{ClozeMaster}: {Fuzzing} {Rust} {Compiler} by {Harnessing} {LLMs} for {Infilling} {Masked} {Real} {Programs}},
 url = {http://www.computer.org/csdl/proceedings-article/icse/2025/056900a712/251mH1NLq1y},
 urldate = {2025-06-12},
 year = {2025}
}
</rdfs:comment>
        <rdfs:label>gao_clozemaster_2025</rdfs:label>
        <rdfs:seeAlso rdf:resource="http://www.computer.org/csdl/proceedings-article/icse/2025/056900a712/251mH1NLq1y"/>
    </owl:NamedIndividual>
    


    <!-- http://purl.org/ai4st/papers#garg_generative_2023 -->

    <owl:NamedIndividual rdf:about="http://purl.org/ai4st/papers#garg_generative_2023">
        <rdf:type rdf:resource="http://purl.org/ai4st/ontology#ResearchPaper"/>
        <hasLevel rdf:resource="http://purl.org/ai4st/ontology#AI-assisted_selection"/>
        <hasPurpose rdf:resource="http://purl.org/ai4st/ontology#Generate"/>
        <hasTarget rdf:resource="http://purl.org/ai4st/ontology#ERP_system"/>
        <hasTarget rdf:resource="http://purl.org/ai4st/ontology#test_generation"/>
        <hasType rdf:resource="http://purl.org/ai4st/ontology#Generative_AI"/>
        <isAboutResearchTopic rdf:resource="http://purl.org/ai4st/ontology#CSO:Testing_and_Debugging"/>
        <rdfs:comment>@inproceedings{garg_generative_2023,
 address = {Faridabad, India},
 author = {Garg, Anshumaan and Sharma, Dolly},
 booktitle = {2023 {International} {Conference} on {Advances} in {Computation}, {Communication} and {Information} {Technology} ({ICAICCIT})},
 copyright = {http://doi.org/10.15223/policy-029},
 doi = {10.1109/ICAICCIT60255.2023.10466102},
 isbn = {979-8-3503-4438-7},
 month = {November},
 pages = {187--193},
 publisher = {IEEE},
 title = {Generative {AI} for {Software} {Test} {Modelling} with a focus on {ERP} {Software}},
 url = {http://ieeexplore.ieee.org/document/10466102/},
 urldate = {2025-06-12},
 year = {2023}
}
</rdfs:comment>
        <rdfs:label>garg_generative_2023</rdfs:label>
        <rdfs:seeAlso rdf:resource="http://ieeexplore.ieee.org/document/10466102/"/>
    </owl:NamedIndividual>
    


    <!-- http://purl.org/ai4st/papers#garlapati_ai-powered_2024 -->

    <owl:NamedIndividual rdf:about="http://purl.org/ai4st/papers#garlapati_ai-powered_2024">
        <rdf:type rdf:resource="http://purl.org/ai4st/ontology#ResearchPaper"/>
        <hasLevel rdf:resource="http://purl.org/ai4st/ontology#AI-driven_partial_automation"/>
        <hasPurpose rdf:resource="http://purl.org/ai4st/ontology#Generate"/>
        <hasTarget rdf:resource="http://purl.org/stc/terms#component_testing"/>
        <hasType rdf:resource="http://purl.org/ai4st/ontology#Generative_AI"/>
        <isAboutResearchTopic rdf:resource="http://purl.org/ai4st/ontology#CSO:Testing_and_Debugging"/>
        <rdfs:comment>@inproceedings{garlapati_ai-powered_2024,
 address = {Bangalore, India},
 author = {Garlapati, Anusha and Satya Sai Muni Parmesh, M N V and {Savitha} and S, Jaisri},
 booktitle = {2024 5th {IEEE} {Global} {Conference} for {Advancement} in {Technology} ({GCAT})},
 copyright = {http://doi.org/10.15223/policy-029},
 doi = {10.1109/GCAT62922.2024.10923987},
 isbn = {979-8-3503-7666-1 979-8-3503-7668-5},
 month = {October},
 pages = {1--5},
 publisher = {IEEE},
 shorttitle = {{AI}-{Powered} {Multi}-{Agent} {Framework} for {Automated} {Unit} {Test} {Case} {Generation}},
 title = {{AI}-{Powered} {Multi}-{Agent} {Framework} for {Automated} {Unit} {Test} {Case} {Generation}: {Enhancing} {Software} {Quality} through {LLM}’s},
 url = {http://ieeexplore.ieee.org/document/10923987/},
 urldate = {2025-06-12},
 year = {2024}
}
</rdfs:comment>
        <rdfs:label>garlapati_ai-powered_2024</rdfs:label>
        <rdfs:seeAlso rdf:resource="http://ieeexplore.ieee.org/document/10923987/"/>
    </owl:NamedIndividual>
    


    <!-- http://purl.org/ai4st/papers#ghimis_river_2020 -->

    <owl:NamedIndividual rdf:about="http://purl.org/ai4st/papers#ghimis_river_2020">
        <rdf:type rdf:resource="http://purl.org/ai4st/ontology#ResearchPaper"/>
        <hasLevel rdf:resource="http://purl.org/ai4st/ontology#AI-driven_full_automation"/>
        <hasPurpose rdf:resource="http://purl.org/ai4st/ontology#Improve"/>
        <hasTarget rdf:resource="http://purl.org/ai4st/ontology#concolic_testing"/>
        <hasTarget rdf:resource="http://purl.org/stc/terms#security_testing"/>
        <hasTarget rdf:resource="http://purl.org/stc/terms#test_automation"/>
        <hasType rdf:resource="http://purl.org/ai4st/ontology#Deep_learning"/>
        <isAboutResearchTopic rdf:resource="http://purl.org/ai4st/ontology#CSO:Testing_and_Debugging"/>
        <rdfs:comment>@inproceedings{ghimis_river_2020,
 address = {Virtual USA},
 author = {Ghimis, Bogdan and Paduraru, Miruna and Stefanescu, Alin},
 booktitle = {Proceedings of the 1st {ACM} {SIGSOFT} {International} {Workshop} on {Languages} and {Tools} for {Next}-{Generation} {Testing}},
 doi = {10.1145/3416504.3424335},
 isbn = {978-1-4503-8123-9},
 language = {en},
 month = {November},
 pages = {13--18},
 publisher = {ACM},
 shorttitle = {{RIVER} 2.0},
 title = {{RIVER} 2.0: an open-source testing framework using {AI} techniques},
 url = {http://dl.acm.org/doi/10.1145/3416504.3424335},
 urldate = {2025-06-12},
 year = {2020}
}
</rdfs:comment>
        <rdfs:label>ghimis_river_2020</rdfs:label>
        <rdfs:seeAlso rdf:resource="http://dl.acm.org/doi/10.1145/3416504.3424335"/>
    </owl:NamedIndividual>
    


    <!-- http://purl.org/ai4st/papers#hagar_ais_2025 -->

    <owl:NamedIndividual rdf:about="http://purl.org/ai4st/papers#hagar_ais_2025">
        <rdf:type rdf:resource="http://purl.org/ai4st/ontology#ResearchPaper"/>
        <hasLevel rdf:resource="http://purl.org/ai4st/ontology#No_AI_automation"/>
        <hasPurpose rdf:resource="http://purl.org/ai4st/ontology#Understand"/>
        <hasTarget rdf:resource="http://purl.org/stc/terms#test_approach"/>
        <hasType rdf:resource="http://purl.org/ai4st/ontology#Generative_AI"/>
        <isAboutResearchTopic rdf:resource="http://purl.org/ai4st/ontology#CSO:Testing_and_Debugging"/>
        <rdfs:comment>@inproceedings{hagar_ais_2025,
 address = {Naples, Italy},
 author = {Hagar, Jon and Wissink, Tome},
 booktitle = {2025 {IEEE} {International} {Conference} on {Software} {Testing}, {Verification} and {Validation} {Workshops} ({ICSTW})},
 copyright = {http://doi.org/10.15223/policy-029},
 doi = {10.1109/ICSTW64639.2025.10962517},
 isbn = {979-8-3315-3467-7},
 month = {March},
 pages = {194--199},
 publisher = {IEEE},
 title = {{AIs} {Understanding} of {Software} {Test} {Architecture}},
 url = {http://ieeexplore.ieee.org/document/10962517/},
 urldate = {2025-06-12},
 year = {2025}
}
</rdfs:comment>
        <rdfs:label>hagar_ais_2025</rdfs:label>
        <rdfs:seeAlso rdf:resource="http://ieeexplore.ieee.org/document/10962517/"/>
    </owl:NamedIndividual>
    


    <!-- http://purl.org/ai4st/papers#haldar_wip_2024 -->

    <owl:NamedIndividual rdf:about="http://purl.org/ai4st/papers#haldar_wip_2024">
        <rdf:type rdf:resource="http://purl.org/ai4st/ontology#ResearchPaper"/>
        <hasLevel rdf:resource="http://purl.org/ai4st/ontology#No_AI_automation"/>
        <hasPurpose rdf:resource="http://purl.org/ai4st/ontology#Understand"/>
        <hasTarget rdf:resource="http://purl.org/stc/terms#testing"/>
        <hasType rdf:resource="http://purl.org/ai4st/ontology#Generative_AI"/>
        <isAboutResearchTopic rdf:resource="http://purl.org/ai4st/ontology#CSO:Testing_and_Debugging"/>
        <rdfs:comment>@inproceedings{haldar_wip_2024,
 address = {Washington, DC, USA},
 author = {Haldar, Susmita and Pierce, Mary and Capretz, Luiz Fernando},
 booktitle = {2024 {IEEE} {Frontiers} in {Education} {Conference} ({FIE})},
 copyright = {http://doi.org/10.15223/policy-029},
 doi = {10.1109/FIE61694.2024.10893214},
 isbn = {979-8-3503-5150-7},
 month = {October},
 pages = {1--5},
 publisher = {IEEE},
 shorttitle = {{WIP}},
 title = {{WIP}: {Assessing} the {Effectiveness} of {ChatGPT} in {Preparatory} {Testing} {Activities}},
 url = {http://ieeexplore.ieee.org/document/10893214/},
 urldate = {2025-06-12},
 year = {2024}
}
</rdfs:comment>
        <rdfs:label>haldar_wip_2024</rdfs:label>
        <rdfs:seeAlso rdf:resource="http://ieeexplore.ieee.org/document/10893214/"/>
    </owl:NamedIndividual>
    


    <!-- http://purl.org/ai4st/papers#happe_getting_2023 -->

    <owl:NamedIndividual rdf:about="http://purl.org/ai4st/papers#happe_getting_2023">
        <rdf:type rdf:resource="http://purl.org/ai4st/ontology#ResearchPaper"/>
        <hasLevel rdf:resource="http://purl.org/ai4st/ontology#AI-assisted_selection"/>
        <hasPurpose rdf:resource="http://purl.org/ai4st/ontology#Generate"/>
        <hasPurpose rdf:resource="http://purl.org/ai4st/ontology#Understand"/>
        <hasTarget rdf:resource="http://purl.org/ai4st/ontology#penetration_testing"/>
        <hasType rdf:resource="http://purl.org/ai4st/ontology#Generative_AI"/>
        <isAboutResearchTopic rdf:resource="http://purl.org/ai4st/ontology#CSO:Testing_and_Debugging"/>
        <rdfs:comment>@inproceedings{happe_getting_2023,
 address = {San Francisco CA USA},
 author = {Happe, Andreas and Cito, Jürgen},
 booktitle = {Proceedings of the 31st {ACM} {Joint} {European} {Software} {Engineering} {Conference} and {Symposium} on the {Foundations} of {Software} {Engineering}},
 doi = {10.1145/3611643.3613083},
 isbn = {979-8-4007-0327-0},
 language = {en},
 month = {November},
 pages = {2082--2086},
 publisher = {ACM},
 shorttitle = {Getting pwn’d by {AI}},
 title = {Getting pwn’d by {AI}: {Penetration} {Testing} with {Large} {Language} {Models}},
 url = {http://dl.acm.org/doi/10.1145/3611643.3613083},
 urldate = {2025-06-12},
 year = {2023}
}</rdfs:comment>
        <rdfs:label>happe_getting_2023</rdfs:label>
        <rdfs:seeAlso rdf:resource="http://dl.acm.org/doi/10.1145/3611643.3613083"/>
    </owl:NamedIndividual>
    


    <!-- http://purl.org/ai4st/papers#helmy_ai-driven_2024 -->

    <owl:NamedIndividual rdf:about="http://purl.org/ai4st/papers#helmy_ai-driven_2024">
        <rdf:type rdf:resource="http://purl.org/ai4st/ontology#ResearchPaper"/>
        <hasLevel rdf:resource="http://purl.org/ai4st/ontology#AI-assisted_selection"/>
        <hasPurpose rdf:resource="http://purl.org/ai4st/ontology#Generate"/>
        <hasTarget rdf:resource="http://purl.org/stc/terms#component_testing"/>
        <hasType rdf:resource="http://purl.org/ai4st/ontology#Generative_AI"/>
        <isAboutResearchTopic rdf:resource="http://purl.org/ai4st/ontology#CSO:Testing_and_Debugging"/>
        <rdfs:comment>@inproceedings{helmy_ai-driven_2024,
 address = {Cairo, Egypt},
 author = {Helmy, Mona and Sobhy, Omar and ElHusseiny, Farida},
 booktitle = {2024 {International} {Telecommunications} {Conference} ({ITC}-{Egypt})},
 copyright = {http://doi.org/10.15223/policy-029},
 doi = {10.1109/ITC-Egypt61547.2024.10620598},
 isbn = {979-8-3503-5140-8},
 month = {July},
 pages = {1--6},
 publisher = {IEEE},
 shorttitle = {{AI}-{Driven} {Testing}},
 title = {{AI}-{Driven} {Testing}: {Unleashing} {Autonomous} {Systems} for {Superior} {Software} {Quality} {Using} {Generative} {AI}},
 url = {http://ieeexplore.ieee.org/document/10620598/},
 urldate = {2025-06-12},
 year = {2024}
}
</rdfs:comment>
        <rdfs:label>helmy_ai-driven_2024</rdfs:label>
        <rdfs:seeAlso rdf:resource="http://ieeexplore.ieee.org/document/10620598/"/>
    </owl:NamedIndividual>
    


    <!-- http://purl.org/ai4st/papers#hossain_togll_2024 -->

    <owl:NamedIndividual rdf:about="http://purl.org/ai4st/papers#hossain_togll_2024">
        <rdf:type rdf:resource="http://purl.org/ai4st/ontology#ResearchPaper"/>
        <hasLevel rdf:resource="http://purl.org/ai4st/ontology#AI-driven_partial_automation"/>
        <hasPurpose rdf:resource="http://purl.org/ai4st/ontology#Generate"/>
        <hasTarget rdf:resource="http://purl.org/stc/terms#test_oracle"/>
        <hasType rdf:resource="http://purl.org/ai4st/ontology#Generative_AI"/>
        <isAboutResearchTopic rdf:resource="http://purl.org/ai4st/ontology#CSO:Testing_and_Debugging"/>
        <rdfs:comment>@misc{hossain_togll_2024,
 author = {Hossain, Soneya Binta and Dwyer, Matthew},
 doi = {10.48550/arXiv.2405.03786},
 keywords = {Computer Science - Software Engineering},
 month = {December},
 note = {arXiv:2405.03786 [cs]},
 publisher = {arXiv},
 shorttitle = {{TOGLL}},
 title = {{TOGLL}: {Correct} and {Strong} {Test} {Oracle} {Generation} with {LLMs}},
 url = {http://arxiv.org/abs/2405.03786},
 urldate = {2025-06-13},
 year = {2024}
}</rdfs:comment>
        <rdfs:label>hossain_togll_2024</rdfs:label>
        <rdfs:seeAlso rdf:resource="http://arxiv.org/abs/2405.03786"/>
    </owl:NamedIndividual>
    


    <!-- http://purl.org/ai4st/papers#kapoor_ai-assisted_2025 -->

    <owl:NamedIndividual rdf:about="http://purl.org/ai4st/papers#kapoor_ai-assisted_2025">
        <rdf:type rdf:resource="http://purl.org/ai4st/ontology#ResearchPaper"/>
        <hasLevel rdf:resource="http://purl.org/ai4st/ontology#AI-assisted_options"/>
        <hasPurpose rdf:resource="http://purl.org/ai4st/ontology#Generate"/>
        <hasTarget rdf:resource="http://purl.org/stc/terms#GUI_testing"/>
        <hasType rdf:resource="http://purl.org/ai4st/ontology#Deep_learning"/>
        <isAboutResearchTopic rdf:resource="http://purl.org/ai4st/ontology#CSO:Testing_and_Debugging"/>
        <rdfs:comment>@inproceedings{kapoor_ai-assisted_2025,
 address = {Bhilai, India},
 author = {Kapoor, Saurabh},
 booktitle = {2025 {Fifth} {International} {Conference} on {Advances} in {Electrical}, {Computing}, {Communication} and {Sustainable} {Technologies} ({ICAECT})},
 copyright = {http://doi.org/10.15223/policy-029},
 doi = {10.1109/ICAECT63952.2025.10958949},
 isbn = {979-8-3503-5623-6},
 month = {January},
 pages = {1--5},
 publisher = {IEEE},
 title = {{AI}-{Assisted} {Test} {Script} {Generation} for {GUI} {Applications}},
 url = {http://ieeexplore.ieee.org/document/10958949/},
 urldate = {2025-06-12},
 year = {2025}
}
</rdfs:comment>
        <rdfs:label>kapoor_ai-assisted_2025</rdfs:label>
        <rdfs:seeAlso rdf:resource="http://ieeexplore.ieee.org/document/10958949/"/>
    </owl:NamedIndividual>
    


    <!-- http://purl.org/ai4st/papers#kaur_approach_2020 -->

    <owl:NamedIndividual rdf:about="http://purl.org/ai4st/papers#kaur_approach_2020">
        <rdf:type rdf:resource="http://purl.org/ai4st/ontology#ResearchPaper"/>
        <hasLevel rdf:resource="http://purl.org/ai4st/ontology#AI-assisted_options"/>
        <hasPurpose rdf:resource="http://purl.org/ai4st/ontology#Improve"/>
        <hasTarget rdf:resource="http://purl.org/stc/terms#regression_testing"/>
        <hasType rdf:resource="http://purl.org/ai4st/ontology#Swarm_intelligence"/>
        <isAboutResearchTopic rdf:resource="http://purl.org/ai4st/ontology#CSO:Testing_and_Debugging"/>
        <rdfs:comment>@inproceedings{kaur_approach_2020,
 address = {Noida, India},
 author = {Kaur, Amandeep},
 booktitle = {2020 10th {International} {Conference} on {Cloud} {Computing}, {Data} {Science} \&amp; {Engineering} ({Confluence})},
 copyright = {http://ieeexplore.ieee.org/Xplorehelp/downloads/license-information/IEEE.html},
 doi = {10.1109/Confluence47617.2020.9058244},
 isbn = {978-1-7281-2791-0},
 month = {January},
 pages = {649--654},
 publisher = {IEEE},
 title = {An {Approach} {To} {Extract} {Optimal} {Test} {Cases} {Using} {AI}},
 url = {http://ieeexplore.ieee.org/document/9058244/},
 urldate = {2025-06-12},
 year = {2020}
}
</rdfs:comment>
        <rdfs:label>kaur_approach_2020</rdfs:label>
        <rdfs:seeAlso rdf:resource="http://ieeexplore.ieee.org/document/9058244/"/>
    </owl:NamedIndividual>
    


    <!-- http://purl.org/ai4st/papers#leu_reducing_2024 -->

    <owl:NamedIndividual rdf:about="http://purl.org/ai4st/papers#leu_reducing_2024">
        <rdf:type rdf:resource="http://purl.org/ai4st/ontology#ResearchPaper"/>
        <hasLevel rdf:resource="http://purl.org/ai4st/ontology#AI-assisted_options"/>
        <hasPurpose rdf:resource="http://purl.org/ai4st/ontology#Generate"/>
        <hasTarget rdf:resource="http://purl.org/stc/terms#API_testing"/>
        <hasTarget rdf:resource="http://purl.org/stc/terms#test_automation"/>
        <hasType rdf:resource="http://purl.org/ai4st/ontology#Deep_learning"/>
        <isAboutResearchTopic rdf:resource="http://purl.org/ai4st/ontology#CSO:Testing_and_Debugging"/>
        <rdfs:comment xml:lang="inproceedings{leu_reducing_2024,  address = {lisbon portugal},  author = {leu, benjamin and volken, jonas and kropp, martin and dogru, nejdet and anslow, craig and biddle, robert},  booktitle = {proceedings of the 5th {acm}/{ieee} {international} {conference} on {automation} of {software} {test} ({ast} 2024)},  doi = {10.1145/3644032.3644449},  isbn = {979-8-4007-0588-5},  language = {en},  month = {april},  pages = {147--148},  publisher = {acm},  title = {reducing {workload} in {using} {ai}-based {api} {rest} {test} {generation}},  url = {http://dl.acm.org/doi/10.1145/3644032.3644449},  urldate = {2025-06-12},  year = {2024} }"></rdfs:comment>
        <rdfs:label>leu_reducing_2024</rdfs:label>
        <rdfs:seeAlso rdf:resource="http://dl.acm.org/doi/10.1145/3644032.3644449"/>
    </owl:NamedIndividual>
    


    <!-- http://purl.org/ai4st/papers#maia_ai-driven_2024 -->

    <owl:NamedIndividual rdf:about="http://purl.org/ai4st/papers#maia_ai-driven_2024">
        <rdf:type rdf:resource="http://purl.org/ai4st/ontology#ResearchPaper"/>
        <hasLevel rdf:resource="http://purl.org/ai4st/ontology#No_AI_automation"/>
        <hasPurpose rdf:resource="http://purl.org/ai4st/ontology#Understand"/>
        <hasTarget rdf:resource="http://purl.org/stc/terms#acceptance_testing"/>
        <hasType rdf:resource="http://purl.org/ai4st/ontology#Generative_AI"/>
        <isAboutResearchTopic rdf:resource="http://purl.org/ai4st/ontology#CSO:Testing_and_Debugging"/>
        <rdfs:comment>@inproceedings{maia_ai-driven_2024,
 address = {Salvador Bahia Brazil},
 author = {Maia, Caio Jordan De Lima and Aguiar, Yuska Paola Costa},
 booktitle = {Proceedings of the {XXIII} {Brazilian} {Symposium} on {Software} {Quality}},
 doi = {10.1145/3701625.3701691},
 isbn = {979-8-4007-1777-2},
 language = {en},
 month = {November},
 pages = {665--672},
 publisher = {ACM},
 shorttitle = {{AI}-{Driven} {Acceptance} {Testing}},
 title = {{AI}-{Driven} {Acceptance} {Testing}: first insights exploring the educational potential for test analysts},
 url = {http://dl.acm.org/doi/10.1145/3701625.3701691},
 urldate = {2025-06-12},
 year = {2024}
}
</rdfs:comment>
        <rdfs:label>maia_ai-driven_2024</rdfs:label>
        <rdfs:seeAlso rdf:resource="http://dl.acm.org/doi/10.1145/3701625.3701691"/>
    </owl:NamedIndividual>
    


    <!-- http://purl.org/ai4st/papers#martin-lopez_ai-driven_2020 -->

    <owl:NamedIndividual rdf:about="http://purl.org/ai4st/papers#martin-lopez_ai-driven_2020">
        <rdf:type rdf:resource="http://purl.org/ai4st/ontology#ResearchPaper"/>
        <hasLevel rdf:resource="http://purl.org/ai4st/ontology#AI-driven_full_automation"/>
        <hasPurpose rdf:resource="http://purl.org/ai4st/ontology#Generate"/>
        <hasTarget rdf:resource="http://purl.org/stc/terms#API_testing"/>
        <hasType rdf:resource="http://purl.org/ai4st/ontology#Classical_machine_learning"/>
        <isAboutResearchTopic rdf:resource="http://purl.org/ai4st/ontology#CSO:Testing_and_Debugging"/>
        <rdfs:comment>@inproceedings{martin-lopez_ai-driven_2020,
 address = {Seoul South Korea},
 author = {Martin-Lopez, Alberto},
 booktitle = {Proceedings of the {ACM}/{IEEE} 42nd {International} {Conference} on {Software} {Engineering}: {Companion} {Proceedings}},
 doi = {10.1145/3377812.3381388},
 isbn = {978-1-4503-7122-3},
 language = {en},
 month = {June},
 pages = {202--205},
 publisher = {ACM},
 title = {{AI}-driven web {API} testing},
 url = {http://dl.acm.org/doi/10.1145/3377812.3381388},
 urldate = {2025-06-12},
 year = {2020}
}
</rdfs:comment>
        <rdfs:label>martin-lopez_ai-driven_2020</rdfs:label>
        <rdfs:seeAlso rdf:resource="http://dl.acm.org/doi/10.1145/3377812.3381388"/>
    </owl:NamedIndividual>
    


    <!-- http://purl.org/ai4st/papers#mohacsi_ai-based_2021 -->

    <owl:NamedIndividual rdf:about="http://purl.org/ai4st/papers#mohacsi_ai-based_2021">
        <rdf:type rdf:resource="http://purl.org/ai4st/ontology#ResearchPaper"/>
        <hasLevel rdf:resource="http://purl.org/ai4st/ontology#AI-assisted_options"/>
        <hasPurpose rdf:resource="http://purl.org/ai4st/ontology#Improve"/>
        <hasTarget rdf:resource="http://purl.org/stc/terms#test_model"/>
        <hasType rdf:resource="http://purl.org/ai4st/ontology#Classical_machine_learning"/>
        <isAboutResearchTopic rdf:resource="http://purl.org/ai4st/ontology#CSO:Testing_and_Debugging"/>
        <rdfs:comment>@inproceedings{mohacsi_ai-based_2021,
 address = {Honolulu, HI, USA},
 author = {Mohacsi, Stefan and Felderer, Michael},
 booktitle = {2021 {IEEE} {International} {Conference} on {Software} {Analysis}, {Evolution} and {Reengineering} ({SANER})},
 copyright = {http://ieeexplore.ieee.org/Xplorehelp/downloads/license-information/IEEE.html},
 doi = {10.1109/SANER50967.2021.00080},
 isbn = {978-1-7281-9630-5},
 month = {March},
 pages = {636--638},
 publisher = {IEEE},
 title = {{AI}-{Based} {Enhancement} of {Test} {Models} in an {Industrial} {Model}-{Based} {Testing} {Tool}},
 url = {http://ieeexplore.ieee.org/document/9426031/},
 urldate = {2025-06-12},
 year = {2021}
}
</rdfs:comment>
        <rdfs:label>mohacsi_ai-based_2021</rdfs:label>
        <rdfs:seeAlso rdf:resource="http://ieeexplore.ieee.org/document/9426031/"/>
    </owl:NamedIndividual>
    


    <!-- http://purl.org/ai4st/papers#naimi_new_2024 -->

    <owl:NamedIndividual rdf:about="http://purl.org/ai4st/papers#naimi_new_2024">
        <rdf:type rdf:resource="http://purl.org/ai4st/ontology#ResearchPaper"/>
        <hasLevel rdf:resource="http://purl.org/ai4st/ontology#AI-assisted_options"/>
        <hasPurpose rdf:resource="http://purl.org/ai4st/ontology#Generate"/>
        <hasTarget rdf:resource="http://purl.org/stc/terms#model_based_testing"/>
        <hasType rdf:resource="http://purl.org/ai4st/ontology#Generative_AI"/>
        <isAboutResearchTopic rdf:resource="http://purl.org/ai4st/ontology#CSO:Testing_and_Debugging"/>
        <rdfs:comment>@inproceedings{naimi_new_2024,
 address = {Fes, Morocco},
 author = {Naimi, Lahbib and Bouziane, El Mahi and Manaouch, Mohamed and Jakimi, Abdeslam},
 booktitle = {2024 {International} {Conference} on {Circuit}, {Systems} and {Communication} ({ICCSC})},
 copyright = {http://doi.org/10.15223/policy-029},
 doi = {10.1109/ICCSC62074.2024.10616548},
 isbn = {979-8-3503-6530-6},
 month = {June},
 pages = {1--5},
 publisher = {IEEE},
 title = {A new approach for automatic test case generation from use case diagram using {LLMs} and prompt engineering},
 url = {http://ieeexplore.ieee.org/document/10616548/},
 urldate = {2025-06-12},
 year = {2024}
}
</rdfs:comment>
        <rdfs:label>naimi_new_2024</rdfs:label>
        <rdfs:seeAlso rdf:resource="http://ieeexplore.ieee.org/document/10616548/"/>
    </owl:NamedIndividual>
    


    <!-- http://purl.org/ai4st/papers#olmez_automation_2024 -->

    <owl:NamedIndividual rdf:about="http://purl.org/ai4st/papers#olmez_automation_2024">
        <rdf:type rdf:resource="http://purl.org/ai4st/ontology#ResearchPaper"/>
        <hasLevel rdf:resource="http://purl.org/ai4st/ontology#AI-assisted_options"/>
        <hasPurpose rdf:resource="http://purl.org/ai4st/ontology#Generate"/>
        <hasTarget rdf:resource="http://purl.org/stc/terms#test_driven_development"/>
        <hasType rdf:resource="http://purl.org/ai4st/ontology#Deep_learning"/>
        <isAboutResearchTopic rdf:resource="http://purl.org/ai4st/ontology#CSO:Testing_and_Debugging"/>
        <rdfs:comment>@inproceedings{olmez_automation_2024,
 address = {Würzburg, Germany},
 author = {Olmez, Muhammet Mustafa and Gehringer, Edward},
 booktitle = {2024 36th {International} {Conference} on {Software} {Engineering} {Education} and {Training} ({CSEE}\&amp;amp;{T})},
 copyright = {http://doi.org/10.15223/policy-029},
 doi = {10.1109/CSEET62301.2024.10663016},
 isbn = {979-8-3503-7897-9},
 month = {July},
 pages = {1--10},
 publisher = {IEEE},
 title = {Automation of {Test} {Skeletons} {Within} {Test}-{Driven} {Development} {Projects}},
 url = {http://ieeexplore.ieee.org/document/10663016/},
 urldate = {2025-06-12},
 year = {2024}
}
</rdfs:comment>
        <rdfs:label>olmez_automation_2024</rdfs:label>
        <rdfs:seeAlso rdf:resource="http://ieeexplore.ieee.org/document/10663016/"/>
    </owl:NamedIndividual>
    


    <!-- http://purl.org/ai4st/papers#peixoto_effectiveness_2025 -->

    <owl:NamedIndividual rdf:about="http://purl.org/ai4st/papers#peixoto_effectiveness_2025">
        <rdf:type rdf:resource="http://purl.org/ai4st/ontology#ResearchPaper"/>
        <hasLevel rdf:resource="http://purl.org/ai4st/ontology#AI-assisted_options"/>
        <hasPurpose rdf:resource="http://purl.org/ai4st/ontology#Improve"/>
        <hasTarget rdf:resource="http://purl.org/ai4st/ontology#test_verification"/>
        <hasType rdf:resource="http://purl.org/ai4st/ontology#Generative_AI"/>
        <isAboutResearchTopic rdf:resource="http://purl.org/ai4st/ontology#CSO:Testing_and_Debugging"/>
        <rdfs:comment>@inproceedings{peixoto_effectiveness_2025,
 address = {Ottawa, ON, Canada},
 author = {Peixoto, Myron and Baía, Davy and Nascimento, Nathalia and Alencar, Paulo and Fonseca, Baldoino and Ribeiro, Márcio},
 booktitle = {2025 {IEEE}/{ACM} {International} {Workshop} on {Deep} {Learning} for {Testing} and {Testing} for {Deep} {Learning} ({DeepTest})},
 copyright = {http://doi.org/10.15223/policy-029},
 doi = {10.1109/DeepTest66595.2025.00012},
 isbn = {979-8-3315-0190-7},
 month = {May},
 pages = {45--52},
 publisher = {IEEE},
 title = {On the {Effectiveness} of {LLMs} for {Manual} {Test} {Verifications}},
 url = {http://ieeexplore.ieee.org/document/11026915/},
 urldate = {2025-06-12},
 year = {2025}
}
</rdfs:comment>
        <rdfs:label>peixoto_effectiveness_2025</rdfs:label>
        <rdfs:seeAlso rdf:resource="http://ieeexplore.ieee.org/document/11026915/"/>
    </owl:NamedIndividual>
    


    <!-- http://purl.org/ai4st/papers#prasetya_agent-based_2021 -->

    <owl:NamedIndividual rdf:about="http://purl.org/ai4st/papers#prasetya_agent-based_2021">
        <rdf:type rdf:resource="http://purl.org/ai4st/ontology#ResearchPaper"/>
        <hasLevel rdf:resource="http://purl.org/ai4st/ontology#Agentic_AI"/>
        <hasPurpose rdf:resource="http://purl.org/ai4st/ontology#Generate"/>
        <hasTarget rdf:resource="http://purl.org/ai4st/new_terms#visual_testing"/>
        <hasType rdf:resource="http://purl.org/ai4st/ontology#Agentic_AI"/>
        <isAboutResearchTopic rdf:resource="http://purl.org/ai4st/ontology#CSO:Testing_and_Debugging"/>
        <rdfs:comment>@inproceedings{prasetya_agent-based_2021,
 address = {Porto de Galinhas, Brazil},
 author = {Prasetya, I. S. W. B. and Shirzadehhajimahmood, Samira and Ansari, Saba Gholizadeh and Fernandes, Pedro and Prada, Rui},
 booktitle = {2021 {IEEE} {International} {Conference} on {Software} {Testing}, {Verification} and {Validation} {Workshops} ({ICSTW})},
 copyright = {http://doi.org/10.15223/policy-029},
 doi = {10.1109/ICSTW52544.2021.00044},
 isbn = {978-1-6654-4456-9},
 month = {April},
 pages = {213--217},
 publisher = {IEEE},
 title = {An {Agent}-based {Architecture} for {AI}-{Enhanced} {Automated} {Testing} for {XR} {Systems}},
 url = {http://ieeexplore.ieee.org/document/9440175/},
 urldate = {2025-06-12},
 year = {2021}
}</rdfs:comment>
        <rdfs:label>prasetya_agent-based_2021</rdfs:label>
        <rdfs:seeAlso rdf:resource="http://ieeexplore.ieee.org/document/9440175/"/>
    </owl:NamedIndividual>
    


    <!-- http://purl.org/ai4st/papers#primbs_assert5_2025 -->

    <owl:NamedIndividual rdf:about="http://purl.org/ai4st/papers#primbs_assert5_2025">
        <rdf:type rdf:resource="http://purl.org/ai4st/ontology#ResearchPaper"/>
        <hasLevel rdf:resource="http://purl.org/ai4st/ontology#AI-driven_partial_automation"/>
        <hasPurpose rdf:resource="http://purl.org/ai4st/ontology#Generate"/>
        <hasTarget rdf:resource="http://purl.org/ai4st/ontology#assertion"/>
        <hasType rdf:resource="http://purl.org/ai4st/ontology#Generative_AI"/>
        <isAboutResearchTopic rdf:resource="http://purl.org/ai4st/ontology#CSO:Testing_and_Debugging"/>
        <rdfs:comment>@misc{primbs_assert5_2025,
 author = {Primbs, Severin and Fein, Benedikt and Fraser, Gordon},
 doi = {10.1109/AST66626.2025.00008},
 keywords = {Computer Science - Software Engineering},
 month = {February},
 note = {arXiv:2502.02708 [cs]},
 shorttitle = {{AsserT5}},
 title = {{AsserT5}: {Test} {Assertion} {Generation} {Using} a {Fine}-{Tuned} {Code} {Language} {Model}},
 url = {http://arxiv.org/abs/2502.02708},
 urldate = {2025-06-12},
 year = {2025}
}</rdfs:comment>
        <rdfs:label>primbs_assert5_2025</rdfs:label>
        <rdfs:seeAlso rdf:resource="http://arxiv.org/abs/2502.02708"/>
    </owl:NamedIndividual>
    


    <!-- http://purl.org/ai4st/papers#ragel_visual_2023 -->

    <owl:NamedIndividual rdf:about="http://purl.org/ai4st/papers#ragel_visual_2023">
        <rdf:type rdf:resource="http://purl.org/ai4st/ontology#ResearchPaper"/>
        <hasLevel rdf:resource="http://purl.org/ai4st/ontology#AI-assisted_options"/>
        <hasPurpose rdf:resource="http://purl.org/ai4st/ontology#Generate"/>
        <hasTarget rdf:resource="http://purl.org/ai4st/new_terms#visual_testing"/>
        <hasTarget rdf:resource="http://purl.org/stc/terms#test_automation"/>
        <hasType rdf:resource="http://purl.org/ai4st/ontology#Deep_learning"/>
        <isAboutResearchTopic rdf:resource="http://purl.org/ai4st/ontology#CSO:Testing_and_Debugging"/>
        <rdfs:comment>@inproceedings{ragel_visual_2023,
 address = {Coron, Palawan, Philippines},
 author = {Ragel, Ritz Kevin C. and Balahadia, Francis F.},
 booktitle = {2023 {IEEE} 15th {International} {Conference} on {Humanoid}, {Nanotechnology}, {Information} {Technology}, {Communication} and {Control}, {Environment}, and {Management} ({HNICEM})},
 copyright = {http://doi.org/10.15223/policy-029},
 doi = {10.1109/HNICEM60674.2023.10589222},
 isbn = {979-8-3503-8117-7},
 month = {November},
 pages = {1--5},
 publisher = {IEEE},
 shorttitle = {Visual {Test} {Framework}},
 title = {Visual {Test} {Framework}: {Enhancing} {Software} {Test} {Automation} with {Visual} {Artificial} {Intelligence} and {Behavioral} {Driven} {Development}},
 url = {http://ieeexplore.ieee.org/document/10589222/},
 urldate = {2025-06-12},
 year = {2023}
}
</rdfs:comment>
        <rdfs:label>ragel_visual_2023</rdfs:label>
        <rdfs:seeAlso rdf:resource="http://ieeexplore.ieee.org/document/10589222/"/>
    </owl:NamedIndividual>
    


    <!-- http://purl.org/ai4st/papers#samplePaper -->

    <owl:NamedIndividual rdf:about="http://purl.org/ai4st/papers#samplePaper">
        <rdf:type rdf:resource="http://purl.org/ai4st/ontology#ResearchPaper"/>
        <hasLevel rdf:resource="http://purl.org/ai4st/ontology#AI-assisted_selection"/>
        <hasPurpose rdf:resource="http://purl.org/ai4st/ontology#Improve"/>
        <hasPurpose rdf:resource="http://purl.org/ai4st/ontology#Understand"/>
        <hasType rdf:resource="http://purl.org/ai4st/ontology#Deep_learning"/>
        <isAboutResearchTopic rdf:resource="http://purl.org/ai4st/ontology#CSO:Testing_and_Debugging"/>
    </owl:NamedIndividual>
    


    <!-- http://purl.org/ai4st/papers#shirzadehhajimahmood_using_2021 -->

    <owl:NamedIndividual rdf:about="http://purl.org/ai4st/papers#shirzadehhajimahmood_using_2021">
        <rdf:type rdf:resource="http://purl.org/ai4st/ontology#ResearchPaper"/>
        <hasLevel rdf:resource="http://purl.org/ai4st/ontology#AI-driven_full_automation"/>
        <hasPurpose rdf:resource="http://purl.org/ai4st/ontology#Generate"/>
        <hasTarget rdf:resource="http://purl.org/ai4st/ontology#computer_game"/>
        <hasTarget rdf:resource="http://purl.org/stc/terms#test_automation"/>
        <hasType rdf:resource="http://purl.org/ai4st/ontology#Agentic_AI"/>
        <isAboutResearchTopic rdf:resource="http://purl.org/ai4st/ontology#CSO:Testing_and_Debugging"/>
        <rdfs:comment>@inproceedings{shirzadehhajimahmood_using_2021,
 address = {Athens Greece},
 author = {Shirzadehhajimahmood, Samira and Prasetya, I. S. W. B. and Dignum, Frank and Dastani, Mehdi and Keller, Gabriele},
 booktitle = {Proceedings of the 12th {International} {Workshop} on {Automating} {TEST} {Case} {Design}, {Selection}, and {Evaluation}},
 doi = {10.1145/3472672.3473952},
 isbn = {978-1-4503-8623-4},
 language = {en},
 month = {August},
 pages = {1--8},
 publisher = {ACM},
 title = {Using an agent-based approach for robust automated testing of computer games},
 url = {http://dl.acm.org/doi/10.1145/3472672.3473952},
 urldate = {2025-06-12},
 year = {2021}
}</rdfs:comment>
        <rdfs:label>shirzadehhajimahmood_using_2021</rdfs:label>
        <rdfs:seeAlso rdf:resource="http://dl.acm.org/doi/10.1145/3472672.3473952"/>
    </owl:NamedIndividual>
    


    <!-- http://purl.org/ai4st/papers#strandberg_ethical_2021 -->

    <owl:NamedIndividual rdf:about="http://purl.org/ai4st/papers#strandberg_ethical_2021">
        <rdf:type rdf:resource="http://purl.org/ai4st/ontology#ResearchPaper"/>
        <hasLevel rdf:resource="http://purl.org/ai4st/ontology#No_AI_automation"/>
        <hasPurpose rdf:resource="http://purl.org/ai4st/ontology#Understand"/>
        <hasTarget rdf:resource="http://purl.org/ai4st/ontology#ethics"/>
        <hasTarget rdf:resource="http://purl.org/ai4st/ontology#test_selection"/>
        <hasType rdf:resource="http://purl.org/ai4st/ontology#Generative_AI"/>
        <isAboutResearchTopic rdf:resource="http://purl.org/ai4st/ontology#CSO:Testing_and_Debugging"/>
        <rdfs:comment>@inproceedings{strandberg_ethical_2021,
 address = {Oxford, United Kingdom},
 author = {Strandberg, Per Erik and Frasheri, Mirgita and Enoiu, Eduard Paul},
 booktitle = {2021 {IEEE} {International} {Conference} on {Artificial} {Intelligence} {Testing} ({AITest})},
 copyright = {http://ieeexplore.ieee.org/Xplorehelp/downloads/license-information/IEEE.html},
 doi = {10.1109/AITEST52744.2021.00025},
 isbn = {978-1-6654-3481-2},
 month = {August},
 pages = {83--84},
 publisher = {IEEE},
 title = {Ethical {AI}-{Powered} {Regression} {Test} {Selection}},
 url = {http://ieeexplore.ieee.org/document/9564367/},
 urldate = {2025-06-12},
 year = {2021}
}</rdfs:comment>
        <rdfs:label>strandberg_ethical_2021</rdfs:label>
        <rdfs:seeAlso rdf:resource="http://ieeexplore.ieee.org/document/9564367/"/>
    </owl:NamedIndividual>
    


    <!-- http://purl.org/ai4st/papers#wang_deep_2024 -->

    <owl:NamedIndividual rdf:about="http://purl.org/ai4st/papers#wang_deep_2024">
        <rdf:type rdf:resource="http://purl.org/ai4st/ontology#ResearchPaper"/>
        <hasLevel rdf:resource="http://purl.org/ai4st/ontology#AI-assisted_options"/>
        <hasPurpose rdf:resource="http://purl.org/ai4st/ontology#Generate"/>
        <hasTarget rdf:resource="http://purl.org/ai4st/ontology#assertion"/>
        <hasType rdf:resource="http://purl.org/ai4st/ontology#Deep_learning"/>
        <isAboutResearchTopic rdf:resource="http://purl.org/ai4st/ontology#CSO:Testing_and_Debugging"/>
        <rdfs:comment>@inproceedings{wang_deep_2024,
 address = {Lisbon Portugal},
 author = {Wang, Hailong and Xu, Tongtong and Wang, Bei},
 booktitle = {Proceedings of the 2024 {IEEE}/{ACM} {First} {International} {Conference} on {AI} {Foundation} {Models} and {Software} {Engineering}},
 doi = {10.1145/3650105.3652293},
 isbn = {979-8-4007-0609-7},
 language = {en},
 month = {April},
 pages = {1--11},
 publisher = {ACM},
 title = {Deep {Multiple} {Assertions} {Generation}},
 url = {http://dl.acm.org/doi/10.1145/3650105.3652293},
 urldate = {2025-06-12},
 year = {2024}
}
</rdfs:comment>
        <rdfs:label>wang_deep_2024</rdfs:label>
        <rdfs:seeAlso rdf:resource="http://dl.acm.org/doi/10.1145/3650105.3652293"/>
    </owl:NamedIndividual>
    


    <!-- http://purl.org/ai4st/papers#yao_bugblitz-ai_2024 -->

    <owl:NamedIndividual rdf:about="http://purl.org/ai4st/papers#yao_bugblitz-ai_2024">
        <rdf:type rdf:resource="http://purl.org/ai4st/ontology#ResearchPaper"/>
        <hasLevel rdf:resource="http://purl.org/ai4st/ontology#AI-driven_partial_automation"/>
        <hasPurpose rdf:resource="http://purl.org/ai4st/ontology#Generate"/>
        <hasTarget rdf:resource="http://purl.org/stc/terms#test_report"/>
        <hasType rdf:resource="http://purl.org/ai4st/ontology#Generative_AI"/>
        <isAboutResearchTopic rdf:resource="http://purl.org/ai4st/ontology#CSO:Testing_and_Debugging"/>
        <rdfs:comment>@inproceedings{yao_bugblitz-ai_2024,
 address = {Changsha, China},
 author = {Yao, Yi and Wang, Jun and Hu, Yabai and Wang, Lifeng and Zhou, Yi and Chen, Jack and Gai, Xuming and Wang, Zhenming and Liu, Wenjun},
 booktitle = {2024 {IEEE} 15th {International} {Conference} on {Software} {Engineering} and {Service} {Science} ({ICSESS})},
 copyright = {http://doi.org/10.15223/policy-029},
 doi = {10.1109/ICSESS62520.2024.10719045},
 isbn = {979-8-3503-8916-6},
 month = {September},
 pages = {57--63},
 publisher = {IEEE},
 shorttitle = {{BugBlitz}-{AI}},
 title = {{BugBlitz}-{AI}: {An} {Intelligent} {QA} {Assistant}},
 url = {http://ieeexplore.ieee.org/document/10719045/},
 urldate = {2025-06-12},
 year = {2024}
}</rdfs:comment>
        <rdfs:label>yao_bugblitz-ai_2024</rdfs:label>
        <rdfs:seeAlso rdf:resource="http://ieeexplore.ieee.org/document/10719045/"/>
    </owl:NamedIndividual>
    


    <!-- http://purl.org/ai4st/papers#zhang_new_2024 -->

    <owl:NamedIndividual rdf:about="http://purl.org/ai4st/papers#zhang_new_2024">
        <rdf:type rdf:resource="http://purl.org/ai4st/ontology#ResearchPaper"/>
        <hasLevel rdf:resource="http://purl.org/ai4st/ontology#AI-driven_full_automation"/>
        <hasPurpose rdf:resource="http://purl.org/ai4st/ontology#Generate"/>
        <hasTarget rdf:resource="http://purl.org/ai4st/ontology#test_generation"/>
        <hasTarget rdf:resource="http://purl.org/stc/terms#test_automation"/>
        <hasType rdf:resource="http://purl.org/ai4st/ontology#Classical_machine_learning"/>
        <hasType rdf:resource="http://purl.org/ai4st/ontology#Deep_learning"/>
        <isAboutResearchTopic rdf:resource="http://purl.org/ai4st/ontology#CSO:Testing_and_Debugging"/>
        <rdfs:comment>@inproceedings{zhang_new_2024,
 address = {Wuhu, China},
 author = {Zhang, Yuli},
 booktitle = {2024 5th {International} {Conference} on {Artificial} {Intelligence} and {Computer} {Engineering} ({ICAICE})},
 copyright = {http://doi.org/10.15223/policy-029},
 doi = {10.1109/ICAICE63571.2024.10863866},
 isbn = {979-8-3315-2891-1},
 month = {November},
 pages = {806--810},
 publisher = {IEEE},
 title = {New {Approaches} to {Automated} {Software} {Testing} {Based} on {Artificial} {Intelligence}},
 url = {http://ieeexplore.ieee.org/document/10863866/},
 urldate = {2025-06-12},
 year = {2024}
}
</rdfs:comment>
        <rdfs:label>zhang_new_2024</rdfs:label>
        <rdfs:seeAlso rdf:resource="http://ieeexplore.ieee.org/document/10863866/"/>
    </owl:NamedIndividual>
    


    <!-- http://purl.org/ai4st/papers#zimmermann_gui-based_2023 -->

    <owl:NamedIndividual rdf:about="http://purl.org/ai4st/papers#zimmermann_gui-based_2023">
        <rdf:type rdf:resource="http://purl.org/ai4st/ontology#ResearchPaper"/>
        <hasLevel rdf:resource="http://purl.org/ai4st/ontology#AI-driven_full_automation"/>
        <hasPurpose rdf:resource="http://purl.org/ai4st/ontology#Generate"/>
        <hasTarget rdf:resource="http://purl.org/ai4st/ontology#Web_application"/>
        <hasTarget rdf:resource="http://purl.org/stc/terms#GUI_testing"/>
        <hasType rdf:resource="http://purl.org/ai4st/ontology#AI-driven_full_automation"/>
        <isAboutResearchTopic rdf:resource="http://purl.org/ai4st/ontology#CSO:Testing_and_Debugging"/>
        <rdfs:comment>@inproceedings{zimmermann_gui-based_2023,
 address = {Luxembourg, Luxembourg},
 author = {Zimmermann, Daniel and Koziolek, Anne},
 booktitle = {2023 38th {IEEE}/{ACM} {International} {Conference} on {Automated} {Software} {Engineering} {Workshops} ({ASEW})},
 copyright = {http://doi.org/10.15223/policy-029},
 doi = {10.1109/ASEW60602.2023.00028},
 isbn = {979-8-3503-3032-8},
 month = {September},
 pages = {171--174},
 publisher = {IEEE},
 shorttitle = {{GUI}-{Based} {Software} {Testing}},
 title = {{GUI}-{Based} {Software} {Testing}: {An} {Automated} {Approach} {Using} {GPT}-4 and {Selenium} {WebDriver}},
 url = {http://ieeexplore.ieee.org/document/10298721/},
 urldate = {2025-06-12},
 year = {2023}
}
</rdfs:comment>
        <rdfs:label>zimmermann_gui-based_2023</rdfs:label>
        <rdfs:seeAlso rdf:resource="http://ieeexplore.ieee.org/document/10298721/"/>
    </owl:NamedIndividual>
    


    <!-- http://purl.org/stc/terms#AI_testing -->

    <rdf:Description rdf:about="http://purl.org/stc/terms#AI_testing">
        <rdf:type rdf:resource="https://purl.org/ai4st/ontology#Target"/>
    </rdf:Description>
    


    <!-- http://purl.org/stc/terms#API_testing -->

    <rdf:Description rdf:about="http://purl.org/stc/terms#API_testing">
        <rdf:type rdf:resource="https://purl.org/ai4st/ontology#Target"/>
    </rdf:Description>
    


    <!-- http://purl.org/stc/terms#GUI_testing -->

    <rdf:Description rdf:about="http://purl.org/stc/terms#GUI_testing">
        <rdf:type rdf:resource="https://purl.org/ai4st/ontology#Target"/>
    </rdf:Description>
    


    <!-- http://purl.org/stc/terms#LLM_structural_coverage -->

    <rdf:Description rdf:about="http://purl.org/stc/terms#LLM_structural_coverage">
        <rdf:type rdf:resource="https://purl.org/ai4st/ontology#Target"/>
    </rdf:Description>
    


    <!-- http://purl.org/stc/terms#MBT_modeller -->

    <rdf:Description rdf:about="http://purl.org/stc/terms#MBT_modeller">
        <rdf:type rdf:resource="https://purl.org/ai4st/ontology#Target"/>
    </rdf:Description>
    


    <!-- http://purl.org/stc/terms#N-switch_coverage -->

    <rdf:Description rdf:about="http://purl.org/stc/terms#N-switch_coverage">
        <rdf:type rdf:resource="https://purl.org/ai4st/ontology#Target"/>
    </rdf:Description>
    


    <!-- http://purl.org/stc/terms#Testware -->

    <rdf:Description rdf:about="http://purl.org/stc/terms#Testware">
        <rdf:type rdf:resource="https://purl.org/ai4st/ontology#Target"/>
    </rdf:Description>
    


    <!-- http://purl.org/stc/terms#a_b_testing -->

    <rdf:Description rdf:about="http://purl.org/stc/terms#a_b_testing">
        <rdf:type rdf:resource="https://purl.org/ai4st/ontology#Target"/>
    </rdf:Description>
    


    <!-- http://purl.org/stc/terms#acceptance -->

    <rdf:Description rdf:about="http://purl.org/stc/terms#acceptance">
        <rdf:type rdf:resource="https://purl.org/ai4st/ontology#Target"/>
    </rdf:Description>
    


    <!-- http://purl.org/stc/terms#acceptance_criteria -->

    <rdf:Description rdf:about="http://purl.org/stc/terms#acceptance_criteria">
        <rdf:type rdf:resource="https://purl.org/ai4st/ontology#Target"/>
    </rdf:Description>
    


    <!-- http://purl.org/stc/terms#acceptance_test-driven_development -->

    <rdf:Description rdf:about="http://purl.org/stc/terms#acceptance_test-driven_development">
        <rdf:type rdf:resource="https://purl.org/ai4st/ontology#Target"/>
    </rdf:Description>
    


    <!-- http://purl.org/stc/terms#acceptance_testing -->

    <rdf:Description rdf:about="http://purl.org/stc/terms#acceptance_testing">
        <rdf:type rdf:resource="https://purl.org/ai4st/ontology#Target"/>
    </rdf:Description>
    


    <!-- http://purl.org/stc/terms#accessibility_testing -->

    <rdf:Description rdf:about="http://purl.org/stc/terms#accessibility_testing">
        <rdf:type rdf:resource="https://purl.org/ai4st/ontology#Target"/>
    </rdf:Description>
    


    <!-- http://purl.org/stc/terms#ad_hoc_testing -->

    <rdf:Description rdf:about="http://purl.org/stc/terms#ad_hoc_testing">
        <rdf:type rdf:resource="https://purl.org/ai4st/ontology#Target"/>
    </rdf:Description>
    


    <!-- http://purl.org/stc/terms#adversarial_testing -->

    <rdf:Description rdf:about="http://purl.org/stc/terms#adversarial_testing">
        <rdf:type rdf:resource="https://purl.org/ai4st/ontology#Target"/>
    </rdf:Description>
    


    <!-- http://purl.org/stc/terms#agile_software_development -->

    <rdf:Description rdf:about="http://purl.org/stc/terms#agile_software_development">
        <rdf:type rdf:resource="https://purl.org/ai4st/ontology#Target"/>
    </rdf:Description>
    


    <!-- http://purl.org/stc/terms#agile_test_leader -->

    <rdf:Description rdf:about="http://purl.org/stc/terms#agile_test_leader">
        <rdf:type rdf:resource="https://purl.org/ai4st/ontology#Target"/>
    </rdf:Description>
    


    <!-- http://purl.org/stc/terms#agile_test_team_leader -->

    <rdf:Description rdf:about="http://purl.org/stc/terms#agile_test_team_leader">
        <rdf:type rdf:resource="https://purl.org/ai4st/ontology#Target"/>
    </rdf:Description>
    


    <!-- http://purl.org/stc/terms#alpha_testing -->

    <rdf:Description rdf:about="http://purl.org/stc/terms#alpha_testing">
        <rdf:type rdf:resource="https://purl.org/ai4st/ontology#Target"/>
    </rdf:Description>
    


    <!-- http://purl.org/stc/terms#architectural_design -->

    <rdf:Description rdf:about="http://purl.org/stc/terms#architectural_design">
        <rdf:type rdf:resource="https://purl.org/ai4st/ontology#Target"/>
    </rdf:Description>
    


    <!-- http://purl.org/stc/terms#automated_testing -->

    <rdf:Description rdf:about="http://purl.org/stc/terms#automated_testing">
        <rdf:type rdf:resource="https://purl.org/ai4st/ontology#Target"/>
    </rdf:Description>
    


    <!-- http://purl.org/stc/terms#back-to-back_testing -->

    <rdf:Description rdf:about="http://purl.org/stc/terms#back-to-back_testing">
        <rdf:type rdf:resource="https://purl.org/ai4st/ontology#Target"/>
    </rdf:Description>
    


    <!-- http://purl.org/stc/terms#base_choice_coverage -->

    <rdf:Description rdf:about="http://purl.org/stc/terms#base_choice_coverage">
        <rdf:type rdf:resource="https://purl.org/ai4st/ontology#Target"/>
    </rdf:Description>
    


    <!-- http://purl.org/stc/terms#basic_concepts -->

    <rdf:Description rdf:about="http://purl.org/stc/terms#basic_concepts">
        <rdf:type rdf:resource="https://purl.org/ai4st/ontology#Target"/>
    </rdf:Description>
    


    <!-- http://purl.org/stc/terms#behavior-driven_development -->

    <rdf:Description rdf:about="http://purl.org/stc/terms#behavior-driven_development">
        <rdf:type rdf:resource="https://purl.org/ai4st/ontology#Target"/>
    </rdf:Description>
    


    <!-- http://purl.org/stc/terms#beta_testing -->

    <rdf:Description rdf:about="http://purl.org/stc/terms#beta_testing">
        <rdf:type rdf:resource="https://purl.org/ai4st/ontology#Target"/>
    </rdf:Description>
    


    <!-- http://purl.org/stc/terms#black_box_test_technique -->

    <rdf:Description rdf:about="http://purl.org/stc/terms#black_box_test_technique">
        <rdf:type rdf:resource="https://purl.org/ai4st/ontology#Target"/>
    </rdf:Description>
    


    <!-- http://purl.org/stc/terms#boundary_value_analysis -->

    <rdf:Description rdf:about="http://purl.org/stc/terms#boundary_value_analysis">
        <rdf:type rdf:resource="https://purl.org/ai4st/ontology#Target"/>
    </rdf:Description>
    


    <!-- http://purl.org/stc/terms#branch_coverage -->

    <rdf:Description rdf:about="http://purl.org/stc/terms#branch_coverage">
        <rdf:type rdf:resource="https://purl.org/ai4st/ontology#Target"/>
    </rdf:Description>
    


    <!-- http://purl.org/stc/terms#branch_testing -->

    <rdf:Description rdf:about="http://purl.org/stc/terms#branch_testing">
        <rdf:type rdf:resource="https://purl.org/ai4st/ontology#Target"/>
    </rdf:Description>
    


    <!-- http://purl.org/stc/terms#change_orientation_in_test_approach -->

    <rdf:Description rdf:about="http://purl.org/stc/terms#change_orientation_in_test_approach">
        <rdf:type rdf:resource="https://purl.org/ai4st/ontology#Target"/>
    </rdf:Description>
    


    <!-- http://purl.org/stc/terms#checklist_based_testing -->

    <rdf:Description rdf:about="http://purl.org/stc/terms#checklist_based_testing">
        <rdf:type rdf:resource="https://purl.org/ai4st/ontology#Target"/>
    </rdf:Description>
    


    <!-- http://purl.org/stc/terms#code -->

    <rdf:Description rdf:about="http://purl.org/stc/terms#code">
        <rdf:type rdf:resource="https://purl.org/ai4st/ontology#Target"/>
    </rdf:Description>
    


    <!-- http://purl.org/stc/terms#coding -->

    <rdf:Description rdf:about="http://purl.org/stc/terms#coding">
        <rdf:type rdf:resource="https://purl.org/ai4st/ontology#Target"/>
    </rdf:Description>
    


    <!-- http://purl.org/stc/terms#compliance_testing -->

    <rdf:Description rdf:about="http://purl.org/stc/terms#compliance_testing">
        <rdf:type rdf:resource="https://purl.org/ai4st/ontology#Target"/>
    </rdf:Description>
    


    <!-- http://purl.org/stc/terms#component_integration_testing -->

    <rdf:Description rdf:about="http://purl.org/stc/terms#component_integration_testing">
        <rdf:type rdf:resource="https://purl.org/ai4st/ontology#Target"/>
    </rdf:Description>
    


    <!-- http://purl.org/stc/terms#component_testing -->

    <rdf:Description rdf:about="http://purl.org/stc/terms#component_testing">
        <rdf:type rdf:resource="https://purl.org/ai4st/ontology#Target"/>
    </rdf:Description>
    


    <!-- http://purl.org/stc/terms#condition_coverage -->

    <rdf:Description rdf:about="http://purl.org/stc/terms#condition_coverage">
        <rdf:type rdf:resource="https://purl.org/ai4st/ontology#Target"/>
    </rdf:Description>
    


    <!-- http://purl.org/stc/terms#configuration_management -->

    <rdf:Description rdf:about="http://purl.org/stc/terms#configuration_management">
        <rdf:type rdf:resource="https://purl.org/ai4st/ontology#Target"/>
    </rdf:Description>
    


    <!-- http://purl.org/stc/terms#confirmation_testing -->

    <rdf:Description rdf:about="http://purl.org/stc/terms#confirmation_testing">
        <rdf:type rdf:resource="https://purl.org/ai4st/ontology#Target"/>
    </rdf:Description>
    


    <!-- http://purl.org/stc/terms#conformance_testing -->

    <rdf:Description rdf:about="http://purl.org/stc/terms#conformance_testing">
        <rdf:type rdf:resource="https://purl.org/ai4st/ontology#Target"/>
    </rdf:Description>
    


    <!-- http://purl.org/stc/terms#continuous_testing -->

    <rdf:Description rdf:about="http://purl.org/stc/terms#continuous_testing">
        <rdf:type rdf:resource="https://purl.org/ai4st/ontology#Target"/>
    </rdf:Description>
    


    <!-- http://purl.org/stc/terms#contract_testing -->

    <rdf:Description rdf:about="http://purl.org/stc/terms#contract_testing">
        <rdf:type rdf:resource="https://purl.org/ai4st/ontology#Target"/>
    </rdf:Description>
    


    <!-- http://purl.org/stc/terms#coverage -->

    <rdf:Description rdf:about="http://purl.org/stc/terms#coverage">
        <rdf:type rdf:resource="https://purl.org/ai4st/ontology#Target"/>
    </rdf:Description>
    


    <!-- http://purl.org/stc/terms#coverage_item -->

    <rdf:Description rdf:about="http://purl.org/stc/terms#coverage_item">
        <rdf:type rdf:resource="https://purl.org/ai4st/ontology#Target"/>
    </rdf:Description>
    


    <!-- http://purl.org/stc/terms#crowd_testing -->

    <rdf:Description rdf:about="http://purl.org/stc/terms#crowd_testing">
        <rdf:type rdf:resource="https://purl.org/ai4st/ontology#Target"/>
    </rdf:Description>
    


    <!-- http://purl.org/stc/terms#data -->

    <rdf:Description rdf:about="http://purl.org/stc/terms#data">
        <rdf:type rdf:resource="https://purl.org/ai4st/ontology#Target"/>
    </rdf:Description>
    


    <!-- http://purl.org/stc/terms#decision_coverage -->

    <rdf:Description rdf:about="http://purl.org/stc/terms#decision_coverage">
        <rdf:type rdf:resource="https://purl.org/ai4st/ontology#Target"/>
    </rdf:Description>
    


    <!-- http://purl.org/stc/terms#decision_table_testing -->

    <rdf:Description rdf:about="http://purl.org/stc/terms#decision_table_testing">
        <rdf:type rdf:resource="https://purl.org/ai4st/ontology#Target"/>
    </rdf:Description>
    


    <!-- http://purl.org/stc/terms#defect -->

    <rdf:Description rdf:about="http://purl.org/stc/terms#defect">
        <rdf:type rdf:resource="https://purl.org/ai4st/ontology#Target"/>
    </rdf:Description>
    


    <!-- http://purl.org/stc/terms#defect_orientation_in_test_approach -->

    <rdf:Description rdf:about="http://purl.org/stc/terms#defect_orientation_in_test_approach">
        <rdf:type rdf:resource="https://purl.org/ai4st/ontology#Target"/>
    </rdf:Description>
    


    <!-- http://purl.org/stc/terms#defect_oriented_metric -->

    <rdf:Description rdf:about="http://purl.org/stc/terms#defect_oriented_metric">
        <rdf:type rdf:resource="https://purl.org/ai4st/ontology#Target"/>
    </rdf:Description>
    


    <!-- http://purl.org/stc/terms#destructive_testing -->

    <rdf:Description rdf:about="http://purl.org/stc/terms#destructive_testing">
        <rdf:type rdf:resource="https://purl.org/ai4st/ontology#Target"/>
    </rdf:Description>
    


    <!-- http://purl.org/stc/terms#detailed_design -->

    <rdf:Description rdf:about="http://purl.org/stc/terms#detailed_design">
        <rdf:type rdf:resource="https://purl.org/ai4st/ontology#Target"/>
    </rdf:Description>
    


    <!-- http://purl.org/stc/terms#development -->

    <rdf:Description rdf:about="http://purl.org/stc/terms#development">
        <rdf:type rdf:resource="https://purl.org/ai4st/ontology#Target"/>
    </rdf:Description>
    


    <!-- http://purl.org/stc/terms#device-based_testing -->

    <rdf:Description rdf:about="http://purl.org/stc/terms#device-based_testing">
        <rdf:type rdf:resource="https://purl.org/ai4st/ontology#Target"/>
    </rdf:Description>
    


    <!-- http://purl.org/stc/terms#domain-specific_test_types -->

    <rdf:Description rdf:about="http://purl.org/stc/terms#domain-specific_test_types">
        <rdf:type rdf:resource="https://purl.org/ai4st/ontology#Target"/>
    </rdf:Description>
    


    <!-- http://purl.org/stc/terms#dynamic_application_security_testing -->

    <rdf:Description rdf:about="http://purl.org/stc/terms#dynamic_application_security_testing">
        <rdf:type rdf:resource="https://purl.org/ai4st/ontology#Target"/>
    </rdf:Description>
    


    <!-- http://purl.org/stc/terms#dynamic_testing -->

    <rdf:Description rdf:about="http://purl.org/stc/terms#dynamic_testing">
        <rdf:type rdf:resource="https://purl.org/ai4st/ontology#Target"/>
    </rdf:Description>
    


    <!-- http://purl.org/stc/terms#each_choice_coverage -->

    <rdf:Description rdf:about="http://purl.org/stc/terms#each_choice_coverage">
        <rdf:type rdf:resource="https://purl.org/ai4st/ontology#Target"/>
    </rdf:Description>
    


    <!-- http://purl.org/stc/terms#end-to-end_testing -->

    <rdf:Description rdf:about="http://purl.org/stc/terms#end-to-end_testing">
        <rdf:type rdf:resource="https://purl.org/ai4st/ontology#Target"/>
    </rdf:Description>
    


    <!-- http://purl.org/stc/terms#entry_criteria -->

    <rdf:Description rdf:about="http://purl.org/stc/terms#entry_criteria">
        <rdf:type rdf:resource="https://purl.org/ai4st/ontology#Target"/>
    </rdf:Description>
    


    <!-- http://purl.org/stc/terms#equivalence_partitioning -->

    <rdf:Description rdf:about="http://purl.org/stc/terms#equivalence_partitioning">
        <rdf:type rdf:resource="https://purl.org/ai4st/ontology#Target"/>
    </rdf:Description>
    


    <!-- http://purl.org/stc/terms#error -->

    <rdf:Description rdf:about="http://purl.org/stc/terms#error">
        <rdf:type rdf:resource="https://purl.org/ai4st/ontology#Target"/>
    </rdf:Description>
    


    <!-- http://purl.org/stc/terms#error_guessing -->

    <rdf:Description rdf:about="http://purl.org/stc/terms#error_guessing">
        <rdf:type rdf:resource="https://purl.org/ai4st/ontology#Target"/>
    </rdf:Description>
    


    <!-- http://purl.org/stc/terms#exhaustive_testing -->

    <rdf:Description rdf:about="http://purl.org/stc/terms#exhaustive_testing">
        <rdf:type rdf:resource="https://purl.org/ai4st/ontology#Target"/>
    </rdf:Description>
    


    <!-- http://purl.org/stc/terms#exit_criteria -->

    <rdf:Description rdf:about="http://purl.org/stc/terms#exit_criteria">
        <rdf:type rdf:resource="https://purl.org/ai4st/ontology#Target"/>
    </rdf:Description>
    


    <!-- http://purl.org/stc/terms#experience-based_testing -->

    <rdf:Description rdf:about="http://purl.org/stc/terms#experience-based_testing">
        <rdf:type rdf:resource="https://purl.org/ai4st/ontology#Target"/>
    </rdf:Description>
    


    <!-- http://purl.org/stc/terms#experience_based_test_metric -->

    <rdf:Description rdf:about="http://purl.org/stc/terms#experience_based_test_metric">
        <rdf:type rdf:resource="https://purl.org/ai4st/ontology#Target"/>
    </rdf:Description>
    


    <!-- http://purl.org/stc/terms#exploratory_testing -->

    <rdf:Description rdf:about="http://purl.org/stc/terms#exploratory_testing">
        <rdf:type rdf:resource="https://purl.org/ai4st/ontology#Target"/>
    </rdf:Description>
    


    <!-- http://purl.org/stc/terms#failure -->

    <rdf:Description rdf:about="http://purl.org/stc/terms#failure">
        <rdf:type rdf:resource="https://purl.org/ai4st/ontology#Target"/>
    </rdf:Description>
    


    <!-- http://purl.org/stc/terms#feature-driven_development -->

    <rdf:Description rdf:about="http://purl.org/stc/terms#feature-driven_development">
        <rdf:type rdf:resource="https://purl.org/ai4st/ontology#Target"/>
    </rdf:Description>
    


    <!-- http://purl.org/stc/terms#formal_review -->

    <rdf:Description rdf:about="http://purl.org/stc/terms#formal_review">
        <rdf:type rdf:resource="https://purl.org/ai4st/ontology#Target"/>
    </rdf:Description>
    


    <!-- http://purl.org/stc/terms#functional_testing -->

    <rdf:Description rdf:about="http://purl.org/stc/terms#functional_testing">
        <rdf:type rdf:resource="https://purl.org/ai4st/ontology#Target"/>
    </rdf:Description>
    


    <!-- http://purl.org/stc/terms#fundamental_test_process -->

    <rdf:Description rdf:about="http://purl.org/stc/terms#fundamental_test_process">
        <rdf:type rdf:resource="https://purl.org/ai4st/ontology#Target"/>
    </rdf:Description>
    


    <!-- http://purl.org/stc/terms#gambling_testing -->

    <rdf:Description rdf:about="http://purl.org/stc/terms#gambling_testing">
        <rdf:type rdf:resource="https://purl.org/ai4st/ontology#Target"/>
    </rdf:Description>
    


    <!-- http://purl.org/stc/terms#grey_box_test_technique -->

    <rdf:Description rdf:about="http://purl.org/stc/terms#grey_box_test_technique">
        <rdf:type rdf:resource="https://purl.org/ai4st/ontology#Target"/>
    </rdf:Description>
    


    <!-- http://purl.org/stc/terms#high_level_test_case -->

    <rdf:Description rdf:about="http://purl.org/stc/terms#high_level_test_case">
        <rdf:type rdf:resource="https://purl.org/ai4st/ontology#Target"/>
    </rdf:Description>
    


    <!-- http://purl.org/stc/terms#incremental_software_development -->

    <rdf:Description rdf:about="http://purl.org/stc/terms#incremental_software_development">
        <rdf:type rdf:resource="https://purl.org/ai4st/ontology#Target"/>
    </rdf:Description>
    


    <!-- http://purl.org/stc/terms#informal_review -->

    <rdf:Description rdf:about="http://purl.org/stc/terms#informal_review">
        <rdf:type rdf:resource="https://purl.org/ai4st/ontology#Target"/>
    </rdf:Description>
    


    <!-- http://purl.org/stc/terms#inspection -->

    <rdf:Description rdf:about="http://purl.org/stc/terms#inspection">
        <rdf:type rdf:resource="https://purl.org/ai4st/ontology#Target"/>
    </rdf:Description>
    


    <!-- http://purl.org/stc/terms#integration -->

    <rdf:Description rdf:about="http://purl.org/stc/terms#integration">
        <rdf:type rdf:resource="https://purl.org/ai4st/ontology#Target"/>
    </rdf:Description>
    


    <!-- http://purl.org/stc/terms#integration_testing -->

    <rdf:Description rdf:about="http://purl.org/stc/terms#integration_testing">
        <rdf:type rdf:resource="https://purl.org/ai4st/ontology#Target"/>
    </rdf:Description>
    


    <!-- http://purl.org/stc/terms#interactive_application_security_testing -->

    <rdf:Description rdf:about="http://purl.org/stc/terms#interactive_application_security_testing">
        <rdf:type rdf:resource="https://purl.org/ai4st/ontology#Target"/>
    </rdf:Description>
    


    <!-- http://purl.org/stc/terms#interface_testing -->

    <rdf:Description rdf:about="http://purl.org/stc/terms#interface_testing">
        <rdf:type rdf:resource="https://purl.org/ai4st/ontology#Target"/>
    </rdf:Description>
    


    <!-- http://purl.org/stc/terms#interoperability_testing -->

    <rdf:Description rdf:about="http://purl.org/stc/terms#interoperability_testing">
        <rdf:type rdf:resource="https://purl.org/ai4st/ontology#Target"/>
    </rdf:Description>
    


    <!-- http://purl.org/stc/terms#iterative_software_development -->

    <rdf:Description rdf:about="http://purl.org/stc/terms#iterative_software_development">
        <rdf:type rdf:resource="https://purl.org/ai4st/ontology#Target"/>
    </rdf:Description>
    


    <!-- http://purl.org/stc/terms#level_test_plan -->

    <rdf:Description rdf:about="http://purl.org/stc/terms#level_test_plan">
        <rdf:type rdf:resource="https://purl.org/ai4st/ontology#Target"/>
    </rdf:Description>
    


    <!-- http://purl.org/stc/terms#load_testing -->

    <rdf:Description rdf:about="http://purl.org/stc/terms#load_testing">
        <rdf:type rdf:resource="https://purl.org/ai4st/ontology#Target"/>
    </rdf:Description>
    


    <!-- http://purl.org/stc/terms#low_level_test_case -->

    <rdf:Description rdf:about="http://purl.org/stc/terms#low_level_test_case">
        <rdf:type rdf:resource="https://purl.org/ai4st/ontology#Target"/>
    </rdf:Description>
    


    <!-- http://purl.org/stc/terms#maintenance -->

    <rdf:Description rdf:about="http://purl.org/stc/terms#maintenance">
        <rdf:type rdf:resource="https://purl.org/ai4st/ontology#Target"/>
    </rdf:Description>
    


    <!-- http://purl.org/stc/terms#maintenance_testing -->

    <rdf:Description rdf:about="http://purl.org/stc/terms#maintenance_testing">
        <rdf:type rdf:resource="https://purl.org/ai4st/ontology#Target"/>
    </rdf:Description>
    


    <!-- http://purl.org/stc/terms#manual_testing -->

    <rdf:Description rdf:about="http://purl.org/stc/terms#manual_testing">
        <rdf:type rdf:resource="https://purl.org/ai4st/ontology#Target"/>
    </rdf:Description>
    


    <!-- http://purl.org/stc/terms#master_test_plan -->

    <rdf:Description rdf:about="http://purl.org/stc/terms#master_test_plan">
        <rdf:type rdf:resource="https://purl.org/ai4st/ontology#Target"/>
    </rdf:Description>
    


    <!-- http://purl.org/stc/terms#math_testing -->

    <rdf:Description rdf:about="http://purl.org/stc/terms#math_testing">
        <rdf:type rdf:resource="https://purl.org/ai4st/ontology#Target"/>
    </rdf:Description>
    


    <!-- http://purl.org/stc/terms#method_orientation_in_test_approach -->

    <rdf:Description rdf:about="http://purl.org/stc/terms#method_orientation_in_test_approach">
        <rdf:type rdf:resource="https://purl.org/ai4st/ontology#Target"/>
    </rdf:Description>
    


    <!-- http://purl.org/stc/terms#metric -->

    <rdf:Description rdf:about="http://purl.org/stc/terms#metric">
        <rdf:type rdf:resource="https://purl.org/ai4st/ontology#Target"/>
    </rdf:Description>
    


    <!-- http://purl.org/stc/terms#mobile_app_testing -->

    <rdf:Description rdf:about="http://purl.org/stc/terms#mobile_app_testing">
        <rdf:type rdf:resource="https://purl.org/ai4st/ontology#Target"/>
    </rdf:Description>
    


    <!-- http://purl.org/stc/terms#model -->

    <rdf:Description rdf:about="http://purl.org/stc/terms#model">
        <rdf:type rdf:resource="https://purl.org/ai4st/ontology#Target"/>
    </rdf:Description>
    


    <!-- http://purl.org/stc/terms#model_based_testing -->

    <rdf:Description rdf:about="http://purl.org/stc/terms#model_based_testing">
        <rdf:type rdf:resource="https://purl.org/ai4st/ontology#Target"/>
    </rdf:Description>
    


    <!-- http://purl.org/stc/terms#model_coverage -->

    <rdf:Description rdf:about="http://purl.org/stc/terms#model_coverage">
        <rdf:type rdf:resource="https://purl.org/ai4st/ontology#Target"/>
    </rdf:Description>
    


    <!-- http://purl.org/stc/terms#model_verification -->

    <rdf:Description rdf:about="http://purl.org/stc/terms#model_verification">
        <rdf:type rdf:resource="https://purl.org/ai4st/ontology#Target"/>
    </rdf:Description>
    


    <!-- http://purl.org/stc/terms#modified_condition_decision_coverage -->

    <rdf:Description rdf:about="http://purl.org/stc/terms#modified_condition_decision_coverage">
        <rdf:type rdf:resource="https://purl.org/ai4st/ontology#Target"/>
    </rdf:Description>
    


    <!-- http://purl.org/stc/terms#multiple_condition_coverage -->

    <rdf:Description rdf:about="http://purl.org/stc/terms#multiple_condition_coverage">
        <rdf:type rdf:resource="https://purl.org/ai4st/ontology#Target"/>
    </rdf:Description>
    


    <!-- http://purl.org/stc/terms#neuron_coverage -->

    <rdf:Description rdf:about="http://purl.org/stc/terms#neuron_coverage">
        <rdf:type rdf:resource="https://purl.org/ai4st/ontology#Target"/>
    </rdf:Description>
    


    <!-- http://purl.org/stc/terms#non-functional_testing -->

    <rdf:Description rdf:about="http://purl.org/stc/terms#non-functional_testing">
        <rdf:type rdf:resource="https://purl.org/ai4st/ontology#Target"/>
    </rdf:Description>
    


    <!-- http://purl.org/stc/terms#operation -->

    <rdf:Description rdf:about="http://purl.org/stc/terms#operation">
        <rdf:type rdf:resource="https://purl.org/ai4st/ontology#Target"/>
    </rdf:Description>
    


    <!-- http://purl.org/stc/terms#oracle_orientation_in_test_approach -->

    <rdf:Description rdf:about="http://purl.org/stc/terms#oracle_orientation_in_test_approach">
        <rdf:type rdf:resource="https://purl.org/ai4st/ontology#Target"/>
    </rdf:Description>
    


    <!-- http://purl.org/stc/terms#pair_testing -->

    <rdf:Description rdf:about="http://purl.org/stc/terms#pair_testing">
        <rdf:type rdf:resource="https://purl.org/ai4st/ontology#Target"/>
    </rdf:Description>
    


    <!-- http://purl.org/stc/terms#peer_review -->

    <rdf:Description rdf:about="http://purl.org/stc/terms#peer_review">
        <rdf:type rdf:resource="https://purl.org/ai4st/ontology#Target"/>
    </rdf:Description>
    


    <!-- http://purl.org/stc/terms#performance_testing -->

    <rdf:Description rdf:about="http://purl.org/stc/terms#performance_testing">
        <rdf:type rdf:resource="https://purl.org/ai4st/ontology#Target"/>
    </rdf:Description>
    


    <!-- http://purl.org/stc/terms#process_improvement -->

    <rdf:Description rdf:about="http://purl.org/stc/terms#process_improvement">
        <rdf:type rdf:resource="https://purl.org/ai4st/ontology#Target"/>
    </rdf:Description>
    


    <!-- http://purl.org/stc/terms#process_orientation_in_software_development -->

    <rdf:Description rdf:about="http://purl.org/stc/terms#process_orientation_in_software_development">
        <rdf:type rdf:resource="https://purl.org/ai4st/ontology#Target"/>
    </rdf:Description>
    


    <!-- http://purl.org/stc/terms#process_orientation_in_test_approach -->

    <rdf:Description rdf:about="http://purl.org/stc/terms#process_orientation_in_test_approach">
        <rdf:type rdf:resource="https://purl.org/ai4st/ontology#Target"/>
    </rdf:Description>
    


    <!-- http://purl.org/stc/terms#project_management -->

    <rdf:Description rdf:about="http://purl.org/stc/terms#project_management">
        <rdf:type rdf:resource="https://purl.org/ai4st/ontology#Target"/>
    </rdf:Description>
    


    <!-- http://purl.org/stc/terms#property-based_testing -->

    <rdf:Description rdf:about="http://purl.org/stc/terms#property-based_testing">
        <rdf:type rdf:resource="https://purl.org/ai4st/ontology#Target"/>
    </rdf:Description>
    


    <!-- http://purl.org/stc/terms#protocol_or_service_testing -->

    <rdf:Description rdf:about="http://purl.org/stc/terms#protocol_or_service_testing">
        <rdf:type rdf:resource="https://purl.org/ai4st/ontology#Target"/>
    </rdf:Description>
    


    <!-- http://purl.org/stc/terms#quality_assurance -->

    <rdf:Description rdf:about="http://purl.org/stc/terms#quality_assurance">
        <rdf:type rdf:resource="https://purl.org/ai4st/ontology#Target"/>
    </rdf:Description>
    


    <!-- http://purl.org/stc/terms#reactive_testing -->

    <rdf:Description rdf:about="http://purl.org/stc/terms#reactive_testing">
        <rdf:type rdf:resource="https://purl.org/ai4st/ontology#Target"/>
    </rdf:Description>
    


    <!-- http://purl.org/stc/terms#regression_testing -->

    <rdf:Description rdf:about="http://purl.org/stc/terms#regression_testing">
        <rdf:type rdf:resource="https://purl.org/ai4st/ontology#Target"/>
    </rdf:Description>
    


    <!-- http://purl.org/stc/terms#regulatory_acceptance_testing -->

    <rdf:Description rdf:about="http://purl.org/stc/terms#regulatory_acceptance_testing">
        <rdf:type rdf:resource="https://purl.org/ai4st/ontology#Target"/>
    </rdf:Description>
    


    <!-- http://purl.org/stc/terms#related_to_role -->

    <rdf:Description rdf:about="http://purl.org/stc/terms#related_to_role">
        <rdf:type rdf:resource="https://purl.org/ai4st/ontology#Target"/>
    </rdf:Description>
    


    <!-- http://purl.org/stc/terms#related_to_team -->

    <rdf:Description rdf:about="http://purl.org/stc/terms#related_to_team">
        <rdf:type rdf:resource="https://purl.org/ai4st/ontology#Target"/>
    </rdf:Description>
    


    <!-- http://purl.org/stc/terms#release -->

    <rdf:Description rdf:about="http://purl.org/stc/terms#release">
        <rdf:type rdf:resource="https://purl.org/ai4st/ontology#Target"/>
    </rdf:Description>
    


    <!-- http://purl.org/stc/terms#requirements-based_testing -->

    <rdf:Description rdf:about="http://purl.org/stc/terms#requirements-based_testing">
        <rdf:type rdf:resource="https://purl.org/ai4st/ontology#Target"/>
    </rdf:Description>
    


    <!-- http://purl.org/stc/terms#requirements_coverage -->

    <rdf:Description rdf:about="http://purl.org/stc/terms#requirements_coverage">
        <rdf:type rdf:resource="https://purl.org/ai4st/ontology#Target"/>
    </rdf:Description>
    


    <!-- http://purl.org/stc/terms#requirements_engineering -->

    <rdf:Description rdf:about="http://purl.org/stc/terms#requirements_engineering">
        <rdf:type rdf:resource="https://purl.org/ai4st/ontology#Target"/>
    </rdf:Description>
    


    <!-- http://purl.org/stc/terms#review -->

    <rdf:Description rdf:about="http://purl.org/stc/terms#review">
        <rdf:type rdf:resource="https://purl.org/ai4st/ontology#Target"/>
    </rdf:Description>
    


    <!-- http://purl.org/stc/terms#risk-based_testing -->

    <rdf:Description rdf:about="http://purl.org/stc/terms#risk-based_testing">
        <rdf:type rdf:resource="https://purl.org/ai4st/ontology#Target"/>
    </rdf:Description>
    


    <!-- http://purl.org/stc/terms#risk_oriented_metric -->

    <rdf:Description rdf:about="http://purl.org/stc/terms#risk_oriented_metric">
        <rdf:type rdf:resource="https://purl.org/ai4st/ontology#Target"/>
    </rdf:Description>
    


    <!-- http://purl.org/stc/terms#safety_testing -->

    <rdf:Description rdf:about="http://purl.org/stc/terms#safety_testing">
        <rdf:type rdf:resource="https://purl.org/ai4st/ontology#Target"/>
    </rdf:Description>
    


    <!-- http://purl.org/stc/terms#scripted_testing -->

    <rdf:Description rdf:about="http://purl.org/stc/terms#scripted_testing">
        <rdf:type rdf:resource="https://purl.org/ai4st/ontology#Target"/>
    </rdf:Description>
    


    <!-- http://purl.org/stc/terms#security_testing -->

    <rdf:Description rdf:about="http://purl.org/stc/terms#security_testing">
        <rdf:type rdf:resource="https://purl.org/ai4st/ontology#Target"/>
    </rdf:Description>
    


    <!-- http://purl.org/stc/terms#sequential_development_model -->

    <rdf:Description rdf:about="http://purl.org/stc/terms#sequential_development_model">
        <rdf:type rdf:resource="https://purl.org/ai4st/ontology#Target"/>
    </rdf:Description>
    


    <!-- http://purl.org/stc/terms#session-based_testing -->

    <rdf:Description rdf:about="http://purl.org/stc/terms#session-based_testing">
        <rdf:type rdf:resource="https://purl.org/ai4st/ontology#Target"/>
    </rdf:Description>
    


    <!-- http://purl.org/stc/terms#software -->

    <rdf:Description rdf:about="http://purl.org/stc/terms#software">
        <rdf:type rdf:resource="https://purl.org/ai4st/ontology#Target"/>
    </rdf:Description>
    


    <!-- http://purl.org/stc/terms#software_development_model -->

    <rdf:Description rdf:about="http://purl.org/stc/terms#software_development_model">
        <rdf:type rdf:resource="https://purl.org/ai4st/ontology#Target"/>
    </rdf:Description>
    


    <!-- http://purl.org/stc/terms#software_engineering -->

    <rdf:Description rdf:about="http://purl.org/stc/terms#software_engineering">
        <rdf:type rdf:resource="https://purl.org/ai4st/ontology#Target"/>
    </rdf:Description>
    


    <!-- http://purl.org/stc/terms#software_engineering_activity -->

    <rdf:Description rdf:about="http://purl.org/stc/terms#software_engineering_activity">
        <rdf:type rdf:resource="https://purl.org/ai4st/ontology#Target"/>
    </rdf:Description>
    


    <!-- http://purl.org/stc/terms#software_engineering_concepts -->

    <rdf:Description rdf:about="http://purl.org/stc/terms#software_engineering_concepts">
        <rdf:type rdf:resource="https://purl.org/ai4st/ontology#Target"/>
    </rdf:Description>
    


    <!-- http://purl.org/stc/terms#software_lifecycle -->

    <rdf:Description rdf:about="http://purl.org/stc/terms#software_lifecycle">
        <rdf:type rdf:resource="https://purl.org/ai4st/ontology#Target"/>
    </rdf:Description>
    


    <!-- http://purl.org/stc/terms#software_testing_concepts -->

    <rdf:Description rdf:about="http://purl.org/stc/terms#software_testing_concepts">
        <rdf:type rdf:resource="https://purl.org/ai4st/ontology#Target"/>
    </rdf:Description>
    


    <!-- http://purl.org/stc/terms#specialist_tester -->

    <rdf:Description rdf:about="http://purl.org/stc/terms#specialist_tester">
        <rdf:type rdf:resource="https://purl.org/ai4st/ontology#Target"/>
    </rdf:Description>
    


    <!-- http://purl.org/stc/terms#specification_coverage -->

    <rdf:Description rdf:about="http://purl.org/stc/terms#specification_coverage">
        <rdf:type rdf:resource="https://purl.org/ai4st/ontology#Target"/>
    </rdf:Description>
    


    <!-- http://purl.org/stc/terms#state_transition_testing -->

    <rdf:Description rdf:about="http://purl.org/stc/terms#state_transition_testing">
        <rdf:type rdf:resource="https://purl.org/ai4st/ontology#Target"/>
    </rdf:Description>
    


    <!-- http://purl.org/stc/terms#statement_coverage -->

    <rdf:Description rdf:about="http://purl.org/stc/terms#statement_coverage">
        <rdf:type rdf:resource="https://purl.org/ai4st/ontology#Target"/>
    </rdf:Description>
    


    <!-- http://purl.org/stc/terms#statement_testing -->

    <rdf:Description rdf:about="http://purl.org/stc/terms#statement_testing">
        <rdf:type rdf:resource="https://purl.org/ai4st/ontology#Target"/>
    </rdf:Description>
    


    <!-- http://purl.org/stc/terms#static_analysis -->

    <rdf:Description rdf:about="http://purl.org/stc/terms#static_analysis">
        <rdf:type rdf:resource="https://purl.org/ai4st/ontology#Target"/>
    </rdf:Description>
    


    <!-- http://purl.org/stc/terms#static_application_security_testing -->

    <rdf:Description rdf:about="http://purl.org/stc/terms#static_application_security_testing">
        <rdf:type rdf:resource="https://purl.org/ai4st/ontology#Target"/>
    </rdf:Description>
    


    <!-- http://purl.org/stc/terms#static_testing -->

    <rdf:Description rdf:about="http://purl.org/stc/terms#static_testing">
        <rdf:type rdf:resource="https://purl.org/ai4st/ontology#Target"/>
    </rdf:Description>
    


    <!-- http://purl.org/stc/terms#stress_testing -->

    <rdf:Description rdf:about="http://purl.org/stc/terms#stress_testing">
        <rdf:type rdf:resource="https://purl.org/ai4st/ontology#Target"/>
    </rdf:Description>
    


    <!-- http://purl.org/stc/terms#structural_coverage -->

    <rdf:Description rdf:about="http://purl.org/stc/terms#structural_coverage">
        <rdf:type rdf:resource="https://purl.org/ai4st/ontology#Target"/>
    </rdf:Description>
    


    <!-- http://purl.org/stc/terms#support_processes -->

    <rdf:Description rdf:about="http://purl.org/stc/terms#support_processes">
        <rdf:type rdf:resource="https://purl.org/ai4st/ontology#Target"/>
    </rdf:Description>
    


    <!-- http://purl.org/stc/terms#system_integration_testing -->

    <rdf:Description rdf:about="http://purl.org/stc/terms#system_integration_testing">
        <rdf:type rdf:resource="https://purl.org/ai4st/ontology#Target"/>
    </rdf:Description>
    


    <!-- http://purl.org/stc/terms#system_testing -->

    <rdf:Description rdf:about="http://purl.org/stc/terms#system_testing">
        <rdf:type rdf:resource="https://purl.org/ai4st/ontology#Target"/>
    </rdf:Description>
    


    <!-- http://purl.org/stc/terms#target_orientation_in_software_development -->

    <rdf:Description rdf:about="http://purl.org/stc/terms#target_orientation_in_software_development">
        <rdf:type rdf:resource="https://purl.org/ai4st/ontology#Target"/>
    </rdf:Description>
    


    <!-- http://purl.org/stc/terms#target_orientation_in_test_approach -->

    <rdf:Description rdf:about="http://purl.org/stc/terms#target_orientation_in_test_approach">
        <rdf:type rdf:resource="https://purl.org/ai4st/ontology#Target"/>
    </rdf:Description>
    


    <!-- http://purl.org/stc/terms#technical_review -->

    <rdf:Description rdf:about="http://purl.org/stc/terms#technical_review">
        <rdf:type rdf:resource="https://purl.org/ai4st/ontology#Target"/>
    </rdf:Description>
    


    <!-- http://purl.org/stc/terms#test_activity -->

    <rdf:Description rdf:about="http://purl.org/stc/terms#test_activity">
        <rdf:type rdf:resource="https://purl.org/ai4st/ontology#Target"/>
    </rdf:Description>
    


    <!-- http://purl.org/stc/terms#test_analysis -->

    <rdf:Description rdf:about="http://purl.org/stc/terms#test_analysis">
        <rdf:type rdf:resource="https://purl.org/ai4st/ontology#Target"/>
    </rdf:Description>
    


    <!-- http://purl.org/stc/terms#test_analyst -->

    <rdf:Description rdf:about="http://purl.org/stc/terms#test_analyst">
        <rdf:type rdf:resource="https://purl.org/ai4st/ontology#Target"/>
    </rdf:Description>
    


    <!-- http://purl.org/stc/terms#test_approach -->

    <rdf:Description rdf:about="http://purl.org/stc/terms#test_approach">
        <rdf:type rdf:resource="https://purl.org/ai4st/ontology#Target"/>
        <skos:altLabel xml:lang="en">test architecture</skos:altLabel>
    </rdf:Description>
    


    <!-- http://purl.org/stc/terms#test_architect -->

    <rdf:Description rdf:about="http://purl.org/stc/terms#test_architect">
        <rdf:type rdf:resource="https://purl.org/ai4st/ontology#Target"/>
    </rdf:Description>
    


    <!-- http://purl.org/stc/terms#test_automation -->

    <rdf:Description rdf:about="http://purl.org/stc/terms#test_automation">
        <rdf:type rdf:resource="https://purl.org/ai4st/ontology#Target"/>
    </rdf:Description>
    


    <!-- http://purl.org/stc/terms#test_automation_engineer -->

    <rdf:Description rdf:about="http://purl.org/stc/terms#test_automation_engineer">
        <rdf:type rdf:resource="https://purl.org/ai4st/ontology#Target"/>
    </rdf:Description>
    


    <!-- http://purl.org/stc/terms#test_basis -->

    <rdf:Description rdf:about="http://purl.org/stc/terms#test_basis">
        <rdf:type rdf:resource="https://purl.org/ai4st/ontology#Target"/>
    </rdf:Description>
    


    <!-- http://purl.org/stc/terms#test_case -->

    <rdf:Description rdf:about="http://purl.org/stc/terms#test_case">
        <rdf:type rdf:resource="https://purl.org/ai4st/ontology#Target"/>
    </rdf:Description>
    


    <!-- http://purl.org/stc/terms#test_completion -->

    <rdf:Description rdf:about="http://purl.org/stc/terms#test_completion">
        <rdf:type rdf:resource="https://purl.org/ai4st/ontology#Target"/>
    </rdf:Description>
    


    <!-- http://purl.org/stc/terms#test_completion_report -->

    <rdf:Description rdf:about="http://purl.org/stc/terms#test_completion_report">
        <rdf:type rdf:resource="https://purl.org/ai4st/ontology#Target"/>
    </rdf:Description>
    


    <!-- http://purl.org/stc/terms#test_condition -->

    <rdf:Description rdf:about="http://purl.org/stc/terms#test_condition">
        <rdf:type rdf:resource="https://purl.org/ai4st/ontology#Target"/>
    </rdf:Description>
    


    <!-- http://purl.org/stc/terms#test_control -->

    <rdf:Description rdf:about="http://purl.org/stc/terms#test_control">
        <rdf:type rdf:resource="https://purl.org/ai4st/ontology#Target"/>
    </rdf:Description>
    


    <!-- http://purl.org/stc/terms#test_data -->

    <rdf:Description rdf:about="http://purl.org/stc/terms#test_data">
        <rdf:type rdf:resource="https://purl.org/ai4st/ontology#Target"/>
    </rdf:Description>
    


    <!-- http://purl.org/stc/terms#test_design -->

    <rdf:Description rdf:about="http://purl.org/stc/terms#test_design">
        <rdf:type rdf:resource="https://purl.org/ai4st/ontology#Target"/>
    </rdf:Description>
    


    <!-- http://purl.org/stc/terms#test_designer -->

    <rdf:Description rdf:about="http://purl.org/stc/terms#test_designer">
        <rdf:type rdf:resource="https://purl.org/ai4st/ontology#Target"/>
    </rdf:Description>
    


    <!-- http://purl.org/stc/terms#test_director -->

    <rdf:Description rdf:about="http://purl.org/stc/terms#test_director">
        <rdf:type rdf:resource="https://purl.org/ai4st/ontology#Target"/>
    </rdf:Description>
    


    <!-- http://purl.org/stc/terms#test_driven_development -->

    <rdf:Description rdf:about="http://purl.org/stc/terms#test_driven_development">
        <rdf:type rdf:resource="https://purl.org/ai4st/ontology#Target"/>
    </rdf:Description>
    


    <!-- http://purl.org/stc/terms#test_execution -->

    <rdf:Description rdf:about="http://purl.org/stc/terms#test_execution">
        <rdf:type rdf:resource="https://purl.org/ai4st/ontology#Target"/>
    </rdf:Description>
    


    <!-- http://purl.org/stc/terms#test_first_approach -->

    <rdf:Description rdf:about="http://purl.org/stc/terms#test_first_approach">
        <rdf:type rdf:resource="https://purl.org/ai4st/ontology#Target"/>
    </rdf:Description>
    


    <!-- http://purl.org/stc/terms#test_implementation -->

    <rdf:Description rdf:about="http://purl.org/stc/terms#test_implementation">
        <rdf:type rdf:resource="https://purl.org/ai4st/ontology#Target"/>
    </rdf:Description>
    


    <!-- http://purl.org/stc/terms#test_item -->

    <rdf:Description rdf:about="http://purl.org/stc/terms#test_item">
        <rdf:type rdf:resource="https://purl.org/ai4st/ontology#Target"/>
    </rdf:Description>
    


    <!-- http://purl.org/stc/terms#test_leader -->

    <rdf:Description rdf:about="http://purl.org/stc/terms#test_leader">
        <rdf:type rdf:resource="https://purl.org/ai4st/ontology#Target"/>
    </rdf:Description>
    


    <!-- http://purl.org/stc/terms#test_level -->

    <rdf:Description rdf:about="http://purl.org/stc/terms#test_level">
        <rdf:type rdf:resource="https://purl.org/ai4st/ontology#Target"/>
    </rdf:Description>
    


    <!-- http://purl.org/stc/terms#test_management -->

    <rdf:Description rdf:about="http://purl.org/stc/terms#test_management">
        <rdf:type rdf:resource="https://purl.org/ai4st/ontology#Target"/>
    </rdf:Description>
    


    <!-- http://purl.org/stc/terms#test_manager -->

    <rdf:Description rdf:about="http://purl.org/stc/terms#test_manager">
        <rdf:type rdf:resource="https://purl.org/ai4st/ontology#Target"/>
    </rdf:Description>
    


    <!-- http://purl.org/stc/terms#test_metric -->

    <rdf:Description rdf:about="http://purl.org/stc/terms#test_metric">
        <rdf:type rdf:resource="https://purl.org/ai4st/ontology#Target"/>
    </rdf:Description>
    


    <!-- http://purl.org/stc/terms#test_model -->

    <rdf:Description rdf:about="http://purl.org/stc/terms#test_model">
        <rdf:type rdf:resource="https://purl.org/ai4st/ontology#Target"/>
    </rdf:Description>
    


    <!-- http://purl.org/stc/terms#test_monitoring -->

    <rdf:Description rdf:about="http://purl.org/stc/terms#test_monitoring">
        <rdf:type rdf:resource="https://purl.org/ai4st/ontology#Target"/>
    </rdf:Description>
    


    <!-- http://purl.org/stc/terms#test_object -->

    <rdf:Description rdf:about="http://purl.org/stc/terms#test_object">
        <rdf:type rdf:resource="https://purl.org/ai4st/ontology#Target"/>
    </rdf:Description>
    


    <!-- http://purl.org/stc/terms#test_objective -->

    <rdf:Description rdf:about="http://purl.org/stc/terms#test_objective">
        <rdf:type rdf:resource="https://purl.org/ai4st/ontology#Target"/>
    </rdf:Description>
    


    <!-- http://purl.org/stc/terms#test_oracle -->

    <rdf:Description rdf:about="http://purl.org/stc/terms#test_oracle">
        <rdf:type rdf:resource="https://purl.org/ai4st/ontology#Target"/>
    </rdf:Description>
    


    <!-- http://purl.org/stc/terms#test_plan -->

    <rdf:Description rdf:about="http://purl.org/stc/terms#test_plan">
        <rdf:type rdf:resource="https://purl.org/ai4st/ontology#Target"/>
    </rdf:Description>
    


    <!-- http://purl.org/stc/terms#test_planning -->

    <rdf:Description rdf:about="http://purl.org/stc/terms#test_planning">
        <rdf:type rdf:resource="https://purl.org/ai4st/ontology#Target"/>
    </rdf:Description>
    


    <!-- http://purl.org/stc/terms#test_process -->

    <rdf:Description rdf:about="http://purl.org/stc/terms#test_process">
        <rdf:type rdf:resource="https://purl.org/ai4st/ontology#Target"/>
    </rdf:Description>
    


    <!-- http://purl.org/stc/terms#test_process_group -->

    <rdf:Description rdf:about="http://purl.org/stc/terms#test_process_group">
        <rdf:type rdf:resource="https://purl.org/ai4st/ontology#Target"/>
    </rdf:Description>
    


    <!-- http://purl.org/stc/terms#test_process_improvement -->

    <rdf:Description rdf:about="http://purl.org/stc/terms#test_process_improvement">
        <rdf:type rdf:resource="https://purl.org/ai4st/ontology#Target"/>
        <hasParent rdf:resource="http://purl.org/stc/terms#process_improvement"/>
    </rdf:Description>
    


    <!-- http://purl.org/stc/terms#test_progress_report -->

    <rdf:Description rdf:about="http://purl.org/stc/terms#test_progress_report">
        <rdf:type rdf:resource="https://purl.org/ai4st/ontology#Target"/>
    </rdf:Description>
    


    <!-- http://purl.org/stc/terms#test_report -->

    <rdf:Description rdf:about="http://purl.org/stc/terms#test_report">
        <rdf:type rdf:resource="https://purl.org/ai4st/ontology#Target"/>
    </rdf:Description>
    


    <!-- http://purl.org/stc/terms#test_script -->

    <rdf:Description rdf:about="http://purl.org/stc/terms#test_script">
        <rdf:type rdf:resource="https://purl.org/ai4st/ontology#Target"/>
    </rdf:Description>
    


    <!-- http://purl.org/stc/terms#test_step -->

    <rdf:Description rdf:about="http://purl.org/stc/terms#test_step">
        <rdf:type rdf:resource="https://purl.org/ai4st/ontology#Target"/>
    </rdf:Description>
    


    <!-- http://purl.org/stc/terms#test_suite -->

    <rdf:Description rdf:about="http://purl.org/stc/terms#test_suite">
        <rdf:type rdf:resource="https://purl.org/ai4st/ontology#Target"/>
    </rdf:Description>
    


    <!-- http://purl.org/stc/terms#test_technique -->

    <rdf:Description rdf:about="http://purl.org/stc/terms#test_technique">
        <rdf:type rdf:resource="https://purl.org/ai4st/ontology#Target"/>
    </rdf:Description>
    


    <!-- http://purl.org/stc/terms#test_type -->

    <rdf:Description rdf:about="http://purl.org/stc/terms#test_type">
        <rdf:type rdf:resource="https://purl.org/ai4st/ontology#Target"/>
    </rdf:Description>
    


    <!-- http://purl.org/stc/terms#test_work_force -->

    <rdf:Description rdf:about="http://purl.org/stc/terms#test_work_force">
        <rdf:type rdf:resource="https://purl.org/ai4st/ontology#Target"/>
    </rdf:Description>
    


    <!-- http://purl.org/stc/terms#tester -->

    <rdf:Description rdf:about="http://purl.org/stc/terms#tester">
        <rdf:type rdf:resource="https://purl.org/ai4st/ontology#Target"/>
    </rdf:Description>
    


    <!-- http://purl.org/stc/terms#tester_orientation_in_test_approach -->

    <rdf:Description rdf:about="http://purl.org/stc/terms#tester_orientation_in_test_approach">
        <rdf:type rdf:resource="https://purl.org/ai4st/ontology#Target"/>
    </rdf:Description>
    


    <!-- http://purl.org/stc/terms#testing -->

    <rdf:Description rdf:about="http://purl.org/stc/terms#testing">
        <rdf:type rdf:resource="https://purl.org/ai4st/ontology#Target"/>
    </rdf:Description>
    


    <!-- http://purl.org/stc/terms#testing_in_production -->

    <rdf:Description rdf:about="http://purl.org/stc/terms#testing_in_production">
        <rdf:type rdf:resource="https://purl.org/ai4st/ontology#Target"/>
    </rdf:Description>
    


    <!-- http://purl.org/stc/terms#testing_quadrants -->

    <rdf:Description rdf:about="http://purl.org/stc/terms#testing_quadrants">
        <rdf:type rdf:resource="https://purl.org/ai4st/ontology#Target"/>
    </rdf:Description>
    


    <!-- http://purl.org/stc/terms#usability_testing -->

    <rdf:Description rdf:about="http://purl.org/stc/terms#usability_testing">
        <rdf:type rdf:resource="https://purl.org/ai4st/ontology#Target"/>
    </rdf:Description>
    


    <!-- http://purl.org/stc/terms#user-agent_based_testing -->

    <rdf:Description rdf:about="http://purl.org/stc/terms#user-agent_based_testing">
        <rdf:type rdf:resource="https://purl.org/ai4st/ontology#Target"/>
    </rdf:Description>
    


    <!-- http://purl.org/stc/terms#user_acceptance_testing -->

    <rdf:Description rdf:about="http://purl.org/stc/terms#user_acceptance_testing">
        <rdf:type rdf:resource="https://purl.org/ai4st/ontology#Target"/>
    </rdf:Description>
    


    <!-- http://purl.org/stc/terms#validation -->

    <rdf:Description rdf:about="http://purl.org/stc/terms#validation">
        <rdf:type rdf:resource="https://purl.org/ai4st/ontology#Target"/>
    </rdf:Description>
    


    <!-- http://purl.org/stc/terms#verification -->

    <rdf:Description rdf:about="http://purl.org/stc/terms#verification">
        <rdf:type rdf:resource="https://purl.org/ai4st/ontology#Target"/>
    </rdf:Description>
    


    <!-- http://purl.org/stc/terms#walkthrough -->

    <rdf:Description rdf:about="http://purl.org/stc/terms#walkthrough">
        <rdf:type rdf:resource="https://purl.org/ai4st/ontology#Target"/>
    </rdf:Description>
    


    <!-- http://purl.org/stc/terms#white_box_test_technique -->

    <rdf:Description rdf:about="http://purl.org/stc/terms#white_box_test_technique">
        <rdf:type rdf:resource="https://purl.org/ai4st/ontology#Target"/>
    </rdf:Description>
    


    <!-- 
    ///////////////////////////////////////////////////////////////////////////////////////
    //
    // Annotations
    //
    ///////////////////////////////////////////////////////////////////////////////////////
     -->

    <rdf:Description rdf:about="http://purl.org/stc/ontology#test_approach">
        <skos:altLabel>test architecture</skos:altLabel>
    </rdf:Description>
</rdf:RDF>



<!-- Generated by the OWL API (version 4.5.29.2024-05-13T12:11:03Z) https://github.com/owlcs/owlapi -->

